theory/JITFix_aux.thy
@@ -1,0 +1,450 @@
+theory JITFix_aux
+  imports JITFlattern JITFix_prob JITFix_def
+begin
+
+lemma length_of_decoded_instr1:
+  "x64_decode xpc l_bin0 = Some(sz, Pcmpq_rr src dst) \<Longrightarrow> 
+  sz = 3"
+  sorry
+
+
+
+lemma well_formed_decode_sequence2:
+  "jitper insns = Some lt \<Longrightarrow> 
+  well_formed_prog lt \<Longrightarrow> 
+  jitflat_bpf lt init_second_layer = (l_bin0,l_pc,l_jump) \<Longrightarrow>
+  unat pc < length lt \<and> unat pc \<ge> 0 \<Longrightarrow>
+  xpc = nat (fst (l_pc!(unat pc))) \<Longrightarrow>
+  num = snd (l_pc!(unat pc)) \<Longrightarrow>
+  x64_decode xpc l_bin0 = Some (sz, Pcmpq_rr src dst) \<Longrightarrow> 
+  num = 1"
+  sorry
+
+lemma " x = 100 \<Longrightarrow> of_nat(unat x) = x"
+  by (metis of_nat_unat ucast_id)
+
+lemma " x = 100 \<Longrightarrow> unat((of_nat x)::u64)= x"
+  by simp
+
+lemma hhh:" (let nsp::64 word = xrs (IR SP) - u64_of_memory_chunk M64 in case storev M64 xm (Vptr sp_block nsp) (Vlong (word_of_nat xpc + (1::64 word))) of None \<Rightarrow> Stuck | Some (m'::nat \<Rightarrow> int \<Rightarrow> 8 word option) \<Rightarrow> let rs1::preg \<Rightarrow> 64 word = xrs(IR SP := nsp) in Next (unat n) rs1 m' xss)= exec_call xpc sz M64 xm xss xrs n"
+  apply(unfold exec_call_def)
+  by blast
+
+lemma hh:
+  assumes a0:"flat_bpf_sem 1 (l_bin0,l_pc,l_jump) (pc,xst) = fxst'" and 
+    a1:"snd fxst' = Next xpc'' xrs'' xm'' xss''" and 
+    a2:"jitper insns = Some lt" and 
+    a3:"xst = Next xpc xrs xm xss" and     
+    a4:"jitflat_bpf lt init_second_layer = (l_bin0,l_pc,l_jump)" and 
+    a5:"well_formed_prog lt" and     
+    a6:"unat pc < length lt \<and> unat pc \<ge> 0"
+    shows "\<exists> num fst'. fix_bpf_sem num (l_bin0,l_pc,l_jump) xst = fst' \<and> match_state2 fst' (snd fxst')"
+proof-
+  have "snd fxst' =  snd (let pair = flat_bpf_one_step (l_bin0,l_pc,l_jump) (pc, xst) in flat_bpf_sem 0 (l_bin0,l_pc,l_jump) pair)"
+            using a0 by simp
+  hence b0_1:"snd fxst' =  snd (flat_bpf_one_step (l_bin0,l_pc,l_jump) (pc, xst))" by (metis flat_bpf_sem.simps(1) prod.collapse)
+  have b0_3:"unat pc < length l_pc" using l_pc_length_prop a4 init_second_layer_def
+    by (metis Nat.add_0_right a6 list.size(3)) 
+  have "fxst' = (let pair = flat_bpf_one_step (l_bin0,l_pc,l_jump) (pc, xst) in flat_bpf_sem 0 (l_bin0,l_pc,l_jump) pair)" using a0 by simp
+  hence b0_2:"nat (fst (l_pc!(unat pc))) = xpc" using a1 b0_3 a3 apply(unfold flat_bpf_one_step_def Let_def,simp_all) by(split if_splits,simp_all)   
+
+  thus ?thesis 
+
+ proof(cases "\<exists> sz src dst. x64_decode xpc l_bin0 = Some(sz, Pcmpq_rr src dst)")
+   case True
+      have c0_0:"\<exists> sz src dst. x64_decode xpc l_bin0 = Some(sz, Pcmpq_rr src dst)" using True by simp
+      then obtain sz src dst where c0_1:"x64_decode xpc l_bin0 = Some(sz, Pcmpq_rr src dst)" by auto
+      hence c0_2:"sz = 3" using length_of_decoded_instr1 by simp
+      (*have "\<exists> l. list_in_list l xpc l_bin0 \<and> x64_decode 0 l = Some(sz, Pcmpq_rr src dst)" using c0_1 sorry
+      then obtain l where c0_3:"list_in_list l xpc l_bin0 \<and> x64_decode 0 l = Some(sz, Pcmpq_rr src dst)" by auto*)
+      have c0:"snd fxst' = snd (let num = snd (l_pc!(unat pc)) in 
+        (case x64_decode (xpc+sz) l_bin0 of Some (sz2,Pjcc _ _) \<Rightarrow>
+         (case x64_sem num l_bin0 (Next xpc xrs xm xss) of
+          Stuck \<Rightarrow> (pc, Stuck) | \<comment>\<open> if one step error, stop, it should be impossible \<close>
+          Next xpc1 rs1 m1 ss1 \<Rightarrow> 
+         (case find_target_pc_in_l_pc l_jump (uint pc) of
+                      None \<Rightarrow> (pc, Stuck) |
+                      Some npc \<Rightarrow>
+            if rs1 (CR ZF) = 1 then \<comment>\<open> must JUMP \<close>            
+                ((npc, (Next (nat (fst (l_pc!(unat npc)))) rs1 m1 ss1))) \<comment>\<open> go to the target address in the jited x64 binary \<close>
+            else \<comment>\<open> donot JUMP \<close>
+              (pc+1, (Next (xpc1+sz2) rs1 m1 ss1))
+           ))|
+            _ \<Rightarrow> (pc, Stuck)))" using True a0 b0_1 a3 a6 b0_3 a1 c0_1
+        apply(unfold flat_bpf_one_step_def Let_def,simp_all) 
+        apply(cases "x64_decode xpc l_bin0",simp_all)
+        subgoal for a by(split if_splits,simp_all)
+        done
+
+      let "?num" = "(snd (l_pc!(unat pc)))" 
+      have c0_4:"\<exists> sz2 cond d. x64_decode (xpc + sz) l_bin0 = Some (sz2,Pjcc cond d)" 
+        using c0 a1 apply(cases "x64_decode (xpc + sz) l_bin0",simp_all)
+        subgoal for a apply(cases a,simp_all)
+          subgoal for aa b apply(cases b,simp_all)
+            done
+          done
+        done
+      then obtain sz2 cond d where c0_5:"x64_decode (xpc + sz) l_bin0 = Some (sz2,Pjcc cond d)" by auto
+      have "\<exists> fxst1. fxst1 = x64_sem ?num l_bin0 (Next xpc xrs xm xss)" by fastforce
+      then obtain fxst1 where c1:"fxst1 = x64_sem ?num l_bin0 (Next xpc xrs xm xss)" by auto
+      have c1_1:"fxst1 \<noteq> Stuck" using c0 a1 c1 using c0_4 
+        apply(cases "x64_decode (xpc + sz) l_bin0",simp_all) 
+        apply(cases "x64_sem ?num l_bin0 (Next xpc xrs xm xss)",simp_all) 
+        subgoal for a apply(cases a,simp_all)
+          subgoal for aa b apply(cases b,simp_all)
+            done
+          done
+        done
+
+      hence "\<exists> xpc1 xrs1 xm1 xss1. Next xpc1 xrs1 xm1 xss1 = fxst1"
+        by (metis outcome.exhaust) 
+      then obtain xpc1 xrs1 xm1 xss1 where c2:"Next xpc1 xrs1 xm1 xss1 = fxst1" by auto
+
+      have bn:"find_target_pc_in_l_pc l_jump (uint pc) \<noteq> None"
+      proof(rule ccontr)
+        assume assm:"\<not> (find_target_pc_in_l_pc l_jump (uint pc) \<noteq> None)"
+        hence "snd fxst' = Stuck" using c0 c0_5 c1_1 c1 assm by(cases "x64_sem ?num l_bin0 (Next xpc xrs xm xss)",simp_all) 
+        thus "False" using a1 by auto
+      qed
+
+      have c3_0:"snd fxst' = snd (case find_target_pc_in_l_pc l_jump (uint pc) of
+              None \<Rightarrow> (pc, Stuck) |
+              Some npc \<Rightarrow> if xrs1 (CR ZF) = 1 then \<comment>\<open> must JUMP \<close>
+              ((npc, (Next (nat (fst (l_pc!(unat npc)))) xrs1 xm1 xss1))) \<comment>\<open> go to the target address in the jited x64 binary \<close>
+            else \<comment>\<open> donot JUMP \<close>
+              (pc+1, (Next (xpc1+sz2) xrs1 xm1 xss1)))
+          " using c2 c1 c0 c0_5 apply(cases "x64_decode (xpc+sz) l_bin0",simp_all)
+        by(cases "x64_sem ?num l_bin0 (Next xpc xrs xm xss)",simp_all)
+
+      have c4:"?num = 1" using well_formed_decode_sequence2 a2 a4 a5 a6 b0_2 c0_1 by blast 
+      hence "fxst1 = x64_sem 0 l_bin0 (exec_instr (Pcmpq_rr src dst) sz xpc xrs xm xss)" 
+        using c0_1 c1 c4 a3 by simp
+      hence c5:"fxst1 = (exec_instr (Pcmpq_rr src dst) sz xpc xrs xm xss)" by simp
+
+      have "fix_bpf_sem 2 (l_bin0,l_pc,l_jump) xst = (
+                 let pair = fix_bpf_one_step (l_bin0,l_pc,l_jump) xst in
+                  fix_bpf_sem 1 (l_bin0,l_pc,l_jump) pair)"
+                  by (metis Suc_1 fix_bpf_sem.simps(2)) 
+                
+      hence d0:"fix_bpf_sem 2 (l_bin0,l_pc,l_jump) xst = (let pair = (
+                      ((case x64_decode xpc l_bin0 of 
+                                    Some(sz, Pcall_i imm) \<Rightarrow>
+                                        let v = find_target_pc_in_l_pc2 l_pc (int xpc) 0 in
+                                        (case v of None \<Rightarrow> Stuck | Some pc \<Rightarrow>
+                                        (case find_target_pc_in_l_pc l_jump pc of
+                                          None \<Rightarrow> Stuck |
+                                          Some npc \<Rightarrow>
+                                        exec_instr (Pcall_i (of_int(fst (l_pc!(unat npc))))) sz xpc xrs xm xss)) |
+                                    Some(sz, Pjcc cond d) \<Rightarrow> 
+                                      let v = find_target_pc_in_l_pc2 l_pc (int xpc-3) 0 in
+                                      (case v of None \<Rightarrow> Stuck | Some pc \<Rightarrow>
+                                        (case find_target_pc_in_l_pc l_jump pc of
+                                          None \<Rightarrow> Stuck |
+                                          Some npc \<Rightarrow>
+                                            (exec_instr (Pjcc cond (of_int (fst (l_pc!(unat npc)))-(of_nat (xpc+1)))) sz xpc xrs xm xss))) |
+                                    Some(sz,ins) \<Rightarrow> (exec_instr ins sz xpc xrs xm xss) |
+                                    _ \<Rightarrow> Stuck 
+                  ))) in fix_bpf_sem 1 (l_bin0,l_pc,l_jump) pair)" using fix_bpf_one_step_def a3 by auto
+
+     hence "fix_bpf_sem 2 (l_bin0,l_pc,l_jump) xst = (let pair = exec_instr (Pcmpq_rr src dst) sz xpc xrs xm xss in fix_bpf_sem 1 (l_bin0,l_pc,l_jump) pair)"
+       using d0 a3 c0_1 by auto
+     hence d2:"fix_bpf_sem 2 (l_bin0,l_pc,l_jump) xst = fix_bpf_sem 1 (l_bin0,l_pc,l_jump) fxst1"
+       using c5 by auto
+     have d2_1:"fix_bpf_sem 1 (l_bin0,l_pc,l_jump) fxst1 = (
+                      ((case x64_decode xpc1 l_bin0 of 
+                                    Some(sz, Pcall_i imm) \<Rightarrow>
+                                         let v = find_target_pc_in_l_pc2 l_pc (int xpc1) 0 in
+                                        (case v of None \<Rightarrow> Stuck | Some pc \<Rightarrow>
+                                        (case find_target_pc_in_l_pc l_jump pc of
+                                          None \<Rightarrow> Stuck |
+                                          Some npc \<Rightarrow>
+                                        exec_instr (Pcall_i (of_int(fst (l_pc!(unat npc))))) sz xpc1 xrs1 xm1 xss1)) |
+                                    Some(sz, Pjcc cond d) \<Rightarrow> 
+                                      let v = find_target_pc_in_l_pc2 l_pc (int xpc1-3) 0 in
+                                      (case v of None \<Rightarrow> Stuck | Some pc \<Rightarrow>
+                                        (case find_target_pc_in_l_pc l_jump pc of
+                                          None \<Rightarrow> Stuck |
+                                          Some npc \<Rightarrow>
+                                            (exec_instr (Pjcc cond (of_int (fst (l_pc!(unat npc)))-(of_nat (xpc1+1)))) sz xpc1 xrs1 xm1 xss1))) |
+                                    Some(sz,ins) \<Rightarrow> (exec_instr ins sz xpc1 xrs1 xm1 xss1) |
+                                    _ \<Rightarrow> Stuck 
+                  )))" using c2 fix_bpf_one_step_def by auto
+
+     have d1_0:"nat (fst (l_pc!(unat pc))) = xpc" using a0 a1 a3 flat_bpf_one_step_def apply(cases xst,simp_all) subgoal for x11
+          using b0_2 by fastforce done
+     hence d1:"find_target_pc_in_l_pc2 l_pc (int xpc) 0 = Some (uint pc)" using l_pc_index_corr b0_3 by (metis a6 less_nat_zero_code list.size(3))
+     have d1_3:"sz+xpc =xpc1"  using c2 c0_1 c5 by(unfold exec_instr_def,simp_all)
+     hence d1_1:"int xpc1-3 = int xpc" using c0_2 by simp
+     hence d1_2:"find_target_pc_in_l_pc2 l_pc (int xpc1-3) 0 = Some (uint pc)" using d1_1 d1 by auto
+     have "x64_decode xpc1 l_bin0 = Some (sz2,Pjcc cond d)" 
+       using c0_5 d1_3 by (simp add: add.commute)
+     hence d5:"fix_bpf_sem 1 (l_bin0,l_pc,l_jump) fxst1 = (case find_target_pc_in_l_pc l_jump (uint pc) of
+                                          None \<Rightarrow> Stuck |
+                                          Some npc \<Rightarrow>
+                                            (exec_instr (Pjcc cond (of_int (fst (l_pc!(unat npc)))-(of_nat (xpc1+1)))) sz2 xpc1 xrs1 xm1 xss1))"
+       using c0_5 d1_2 d2_1 c5 d2 d1_3 bn by(cases "x64_decode xpc1 l_bin0",simp_all)
+
+      thus ?thesis
+      proof(cases "xrs1 (CR ZF) = 1")
+        case True
+        have b1:"xrs1 (CR ZF) = 1" using True by simp
+
+                have "\<exists> npc. find_target_pc_in_l_pc l_jump (uint pc) = Some npc" using bn by simp
+                then obtain npc where c3_1:"find_target_pc_in_l_pc l_jump (uint pc) = Some npc" by auto                                 
+                have c3:"snd fxst' = (Next (nat (fst (l_pc!(unat npc)))) xrs1 xm1 xss1)" 
+                  using True c3_0 c3_1 b1 by simp
+
+                have "cond = Cond_e" sorry
+                hence d6:"eval_testcond cond xrs1 = (Some (xrs1 (CR ZF) = 1))" 
+                  using b1 eval_testcond_def by(cases cond,simp_all)
+
+                have d8:"fix_bpf_sem 1 (l_bin0,l_pc,l_jump) fxst1 = (exec_instr (Pjcc cond (of_int (fst (l_pc!(unat npc)))-(of_nat (xpc1+1)))) sz2 xpc1 xrs1 xm1 xss1)" 
+                  using True d5 c3_1 by simp
+                have "fix_bpf_sem 1 (l_bin0,l_pc,l_jump) fxst1  = (case eval_testcond cond xrs1 of Some b \<Rightarrow> 
+                          if b then Next (unat (of_int (fst (l_pc!(unat npc)))-(of_nat (xpc1+1))::i32)+xpc1+1) xrs1 xm1 xss1
+                          else Next (xpc1+sz2) xrs1 xm1 xss1 | 
+                        None \<Rightarrow> Stuck)" using d8 True d6 apply(unfold exec_instr_def,simp_all) done
+                  
+                hence d9:"fix_bpf_sem 1 (l_bin0,l_pc,l_jump) fxst1 = (Next (nat (fst (l_pc!(unat npc)))) xrs1 xm1 xss1)" using d6 True apply(cases "eval_testcond cond xrs1",simp_all)
+                  subgoal for a sorry done
+                hence "fix_bpf_sem 2 (l_bin0,l_pc,l_jump) xst =  (Next (nat (fst (l_pc!(unat npc)))) xrs1 xm1 xss1)" using d2 by auto
+
+                hence "\<exists> num fst'. fix_bpf_sem num (l_bin0,l_pc,l_jump) xst = fst' \<and> match_state2 fst' (snd fxst')" 
+                  using match_state2_def match_mem_def c3 a1 by (smt (verit, ccfv_SIG) outcome.simps(4)) 
+                thus ?thesis by simp
+  
+ next
+   case False
+   have b1:"\<not>(xrs1 (CR ZF) = 1)" using False by simp
+   have b1_1:"snd fxst' = (Next (xpc1+sz2) xrs1 xm1 xss1)" using b1 c3_0 c0_5 bn by fastforce   
+   hence "\<exists> npc. find_target_pc_in_l_pc l_jump (uint pc) = Some npc" using bn by simp
+   then obtain npc where b2:"find_target_pc_in_l_pc l_jump (uint pc) = Some npc" by auto
+   have "cond = Cond_e" sorry
+   hence b2_1:"eval_testcond cond xrs1 = Some False" using b1 by(unfold eval_testcond_def,simp_all)
+   have "fix_bpf_sem 1 (l_bin0,l_pc,l_jump) fxst1 = (exec_instr (Pjcc cond (of_int (fst (l_pc!(unat npc)))-(of_nat (xpc1+1)))) sz2 xpc1 xrs1 xm1 xss1)" using b2 d5 by simp
+   
+   hence b3:"fix_bpf_sem 1 (l_bin0,l_pc,l_jump) fxst1 = (Next (xpc1+sz2) xrs1 xm1 xss1)"  using b2_1 by(unfold exec_instr_def,simp_all) 
+   
+   hence "fix_bpf_sem 2 (l_bin0,l_pc,l_jump) xst = Next (xpc1+sz2) xrs1 xm1 xss1" using b3 a2 d2 by simp
+   hence "\<exists> num fst'. fix_bpf_sem num (l_bin0,l_pc,l_jump) xst = fst' \<and> match_state2 fst' (snd fxst')" 
+   using match_state2_def match_mem_def by (smt (verit, del_insts) b1_1 outcome.simps(4)) 
+
+   then show ?thesis by simp
+ qed
+next
+  case False
+  have b1:"\<not>(\<exists> sz src dst. x64_decode xpc l_bin0 = Some(sz, Pcmpq_rr src dst))" using False by simp
+  then show ?thesis 
+  proof(cases "\<exists> sz imm. x64_decode xpc l_bin0 = Some(sz, Pcall_i imm)")
+    case True
+    have b1:"\<exists> sz imm. x64_decode xpc l_bin0 = Some(sz, Pcall_i imm)" using True by auto
+    then obtain sz imm where b2:"x64_decode xpc l_bin0 = Some(sz, Pcall_i imm)" by auto
+    have c0:"snd fxst' = snd (let num = snd (l_pc!(unat pc)) in case x64_decode xpc l_bin0 of Some(_, Pcall_i _) \<Rightarrow>
+            (case find_target_pc_in_l_pc l_jump (uint pc) of 
+              None \<Rightarrow> (pc, Stuck) |
+              Some npc \<Rightarrow> (let xst_temp = exec_instr (Pcall_i (of_int(fst (l_pc!(unat npc))))) sz xpc xrs xm xss in 
+                  (case xst_temp of Stuck \<Rightarrow> (pc, Stuck) | 
+                                    Next xpc' rs' m' ss' \<Rightarrow> (npc, (Next xpc' rs' m' ss'))))))" 
+      using b0_1 b0_3 b2 a3 b0_2 by(unfold flat_bpf_one_step_def,simp_all)
+    hence c1:"find_target_pc_in_l_pc l_jump (uint pc) \<noteq> None" using a1 b2
+      using split_pairs by fastforce 
+    hence "\<exists> npc. find_target_pc_in_l_pc l_jump (uint pc) = Some npc" by simp
+    then obtain npc where c2:"find_target_pc_in_l_pc l_jump (uint pc) = Some npc" by auto
+    have c3_1:"exec_instr (Pcall_i (of_int(fst (l_pc!(unat npc))))) sz xpc xrs xm xss \<noteq> Stuck" using c2 c0 a1 b2 by fastforce
+    hence c3:"snd fxst' = (case exec_instr (Pcall_i (of_int(fst (l_pc!(unat npc))))) sz xpc xrs xm xss of Next xpc' rs' m' ss' \<Rightarrow> 
+              Next xpc' rs' m' ss')" 
+      using c0 c2 True
+      by (smt (z3) case_prod_conv exec_instr_def hhh instruction.simps(548) option.case_eq_if option.simps(5) outcome.simps(4) split_pairs) 
+     
+    have "Mem.storev M64 xm (Vptr sp_block ((xrs (IR SP))-(u64_of_memory_chunk M64)))  (Vlong (of_nat xpc+1)) \<noteq> None" using exec_call_def c3_1 Let_def
+      by (simp add: storev_stack_some) 
+    hence "\<exists> m'. storev M64 xm (Vptr sp_block ( xrs (IR SP) - u64_of_memory_chunk M64)) (Vlong (of_nat xpc + (1::64 word))) = Some m'" by auto
+    then obtain m' where c3_2:"storev M64 xm (Vptr sp_block ( xrs (IR SP) - u64_of_memory_chunk M64)) (Vlong (of_nat xpc + (1::64 word))) = Some m'" by auto
+    hence c4_0:"exec_instr (Pcall_i (of_int(fst (l_pc!(unat npc))))) sz xpc xrs xm xss = Next (unat (of_int(fst (l_pc!(unat npc))))) (xrs#(IR SP) <- ((xrs (IR SP))-(u64_of_memory_chunk M64))) m' xss" 
+      using c3_2 apply (simp add: exec_call_def,simp_all) sorry
+    have c4_1:"nat (fst (l_pc!(unat npc))) = (unat (of_int(fst (l_pc!(unat npc)))))" sorry
+    hence c4:"snd fxst' = Next (nat (fst (l_pc!(unat npc)))) (xrs#(IR SP) <- ((xrs (IR SP))-(u64_of_memory_chunk M64))) m' xss" 
+      using c3 by (metis c4_0 outcome.simps(4)) 
+
+    have "fix_bpf_sem 1 (l_bin0,l_pc,l_jump) xst = fix_bpf_one_step (l_bin0,l_pc,l_jump) xst" by simp
+    hence d0:"fix_bpf_sem 1 (l_bin0,l_pc,l_jump) xst = 
+                      (let v = find_target_pc_in_l_pc2 l_pc (int xpc) 0 in
+                      (case v of None \<Rightarrow> Stuck | Some pc \<Rightarrow>
+                      (case find_target_pc_in_l_pc l_jump pc of
+                        None \<Rightarrow> Stuck |
+                        Some npc \<Rightarrow>
+                      exec_instr (Pcall_i (of_int(fst (l_pc!(unat npc))))) sz xpc xrs xm xss)))" 
+      using b2 a3 by(unfold fix_bpf_one_step_def,simp_all)
+    
+    let "?imm" = "(of_int(fst (l_pc!(unat npc))))"
+    have d1:"find_target_pc_in_l_pc2 l_pc (int xpc) 0 = Some (uint pc)"
+      by (metis a6 b0_2 b0_3 l_pc_index_corr less_nat_zero_code list.size(3)) 
+    hence d2:"fix_bpf_sem 1 (l_bin0,l_pc,l_jump) xst = exec_instr (Pcall_i ?imm) sz xpc xrs xm xss"
+      using d1 c2 d0 by force
+    hence "fix_bpf_sem 1 (l_bin0,l_pc,l_jump) xst = exec_call xpc sz M64 xm xss xrs ?imm"
+      using exec_instr_def by auto
+    
+    have "fix_bpf_sem 1 (l_bin0,l_pc,l_jump) xst = (
+           (let nsp::64 word = xrs (IR SP) - u64_of_memory_chunk M64 in case storev M64 xm (Vptr sp_block nsp) (Vlong (of_nat xpc + (1::64 word))) of None \<Rightarrow> Stuck | 
+                Some (m'::nat \<Rightarrow> int \<Rightarrow> 8 word option) \<Rightarrow> let rs1::preg \<Rightarrow> 64 word = xrs(IR SP := nsp) in Next (unat ?imm) rs1 m' xss) 
+  )" using exec_call_def of_nat_def of_int_def sorry
+    hence d3:"fix_bpf_sem 1 (l_bin0,l_pc,l_jump) xst = Next (unat (of_int (fst (l_pc ! unat npc)))) (xrs#(IR SP) <- ((xrs (IR SP))-(u64_of_memory_chunk M64))) m' xss"
+      using c3_2 by auto
+
+    have "(unat (of_int (fst (l_pc!(unat npc))))) = nat (fst (l_pc!(unat npc)))" using c4_1 by metis
+    hence "match_state2 (fix_bpf_sem 1 (l_bin0,l_pc,l_jump) xst) (snd fxst')" using match_state2_def match_mem_def d3 c4
+      by (smt (verit, best) outcome.simps(4)) 
+    hence "\<exists> num fst'. fix_bpf_sem num (l_bin0,l_pc,l_jump) xst = fst' \<and> match_state2 fst' (snd fxst')" by blast
+    then show ?thesis by simp
+  next
+    case False
+    have b2:"\<not> (\<exists> sz src dst. x64_decode xpc l_bin0 = Some(sz, Pcmpq_rr src dst)) \<and> \<not> (\<exists> sz imm. x64_decode xpc l_bin0 = Some(sz, Pcall_i imm))" using b1 False by simp
+    then show ?thesis
+    proof(cases "\<exists> sz. x64_decode xpc l_bin0 = Some(sz, Pret_anchor)")
+      case True
+      obtain sz where b2_0:"x64_decode xpc l_bin0 = Some(sz, Pret_anchor)" using True by auto
+      have "\<exists> pc'. fxst' = (pc', Next xpc'' xrs'' xm'' xss'')" using a0 a1
+        by (metis eq_snd_iff) 
+      then obtain pc' where b2_1:"fxst' = (pc', Next xpc'' xrs'' xm'' xss'')" by auto
+      hence "fxst' = (let pair = flat_bpf_one_step (l_bin0,l_pc,l_jump) (pc, xst) in flat_bpf_sem 0 (l_bin0,l_pc,l_jump) pair)"using a0 by simp
+      hence b0_1:"fxst' = flat_bpf_one_step (l_bin0,l_pc,l_jump) (pc, xst)" by (metis flat_bpf_sem.simps(1) prod.collapse)
+      have "\<exists> sz2. x64_decode (xpc+sz) l_bin0 = Some (sz2,Pret)" using b2_0 b2_1 b0_1 a3 b0_3 b0_2 apply(unfold flat_bpf_one_step_def Let_def,simp_all) 
+        apply(cases "x64_decode (xpc + sz) l_bin0",simp_all)
+        subgoal for a apply(cases a,simp_all)
+          subgoal for aa b apply(cases b,simp_all)
+            done
+          done
+        done
+      then obtain sz2 where b2_2:"x64_decode (xpc+sz) l_bin0 = Some (sz2,Pret)" by auto
+      hence c0:"(pc', Next xpc'' xrs'' xm'' xss'') = 
+          (let (pc', ss', caller,fp) = update_stack2 xss in 
+          if find_target_pc_in_l_pc3 l_jump (uint pc) \<noteq> Some (uint pc') then (pc,Stuck) else
+          let rs' = restore_x64_caller xrs caller fp in let xst_temp = exec_instr Pret sz2 (xpc+sz) rs' xm ss' in 
+          (case xst_temp of Stuck \<Rightarrow> (pc,Stuck)| Next xpc1 rs1 m1 ss1 \<Rightarrow> 
+            (if xpc1 = (nat (fst (l_pc!(unat pc')))+1) then (pc',Next xpc1 rs1 m1 ss1) else (pc,Stuck) )))" 
+        using a6 a3 a0 a1 b0_3 b0_2 b2_0 b0_1 b2_1 by(unfold flat_bpf_one_step_def Let_def,simp_all) 
+      
+      let "?ss'" = "(fst(snd(update_stack2 xss)))"
+      let "?rs'" = "(restore_x64_caller xrs (fst(snd(snd(update_stack2 xss)))) (snd(snd(snd(update_stack2 xss)))))"
+      let "?pc'" = "fst (update_stack2 xss)"
+      
+      have cn:"find_target_pc_in_l_pc3 l_jump (uint pc) = Some (uint (?pc'))" using c0 apply(cases "update_stack2 xss",simp_all)
+        subgoal for a b c d apply(split if_splits,simp_all)
+          done
+        done
+
+      have c0_2:"exec_instr Pret sz2 (xpc+sz) ?rs' xm ?ss' \<noteq> Stuck" using c0 cn apply(unfold Let_def,simp_all) apply(cases "update_stack2 xss",simp_all)
+        subgoal for a b c d by fastforce 
+        done
+      hence "\<exists> xpc1 xrs1 xss1 xm1. exec_instr Pret sz2 (xpc+sz) ?rs' xm ?ss' = Next xpc1 xrs1 xss1 xm1"
+        by (meson outcome.exhaust) 
+      then obtain xpc1 xrs1 xss1 xm1 where c0_3:"exec_instr Pret sz2 (xpc+sz) ?rs' xm ?ss' = Next xpc1 xrs1 xss1 xm1" by auto
+      hence "xpc1 = (nat (fst (l_pc!(unat ?pc')))+1)"
+        using c0 cn apply(unfold Let_def,simp_all) apply(cases "update_stack2 xss",simp_all)
+        subgoal for a b c d 
+          by (smt (verit, ccfv_threshold) outcome.distinct(1) outcome.exhaust outcome.simps(4) split_pairs)
+        done
+      hence c0_6:"Next xpc1 xrs1 xss1 xm1 = Next xpc'' xrs'' xm'' xss''"
+          using c0 c0_2 cn c0_3 apply(unfold Let_def,simp_all) 
+          by(cases "update_stack2 xss",simp_all)
+      
+      have c0_4:"exec_instr Pret sz2 (xpc+sz) ?rs' xm ?ss' = (
+          let nsp =  (?rs' (IR SP)) + (u64_of_memory_chunk M64) in
+            case Mem.loadv M64 xm (Vptr sp_block nsp) of
+            None \<Rightarrow> Stuck |
+            Some ra \<Rightarrow> (
+              case ra of
+              Vlong v \<Rightarrow> let rs1 = ?rs'#(IR SP) <- nsp in
+                          Next (unat v) rs1 xm ?ss' |
+              _ \<Rightarrow> Stuck)
+        )" using exec_instr_def by (simp add: exec_ret_def) 
+
+      hence "\<exists> v. Mem.loadv M64 xm (Vptr sp_block ((?rs' (IR SP)) + (u64_of_memory_chunk M64))) = Some (Vlong v)"
+        using c0_3 c0_2
+        by (smt (verit, ccfv_SIG) option.case_eq_if option.collapse val.case(1) val.case(2) val.case(3) val.case(4) val.case(6) val.exhaust) 
+
+      then obtain v where c0_5:"Mem.loadv M64 xm (Vptr sp_block ((?rs' (IR SP)) + (u64_of_memory_chunk M64))) = Some (Vlong v)" by auto
+      
+      hence c0_7:"exec_instr Pret sz2 (xpc+sz) ?rs' xm ?ss' = Next (unat v) (?rs'#(IR SP) <- ((?rs' (IR SP)) + (u64_of_memory_chunk M64))) xm ?ss'" 
+        using c0_4 Let_def by simp
+      hence c1:"snd fxst' = Next (unat v) (?rs'#(IR SP) <- ((?rs' (IR SP)) + (u64_of_memory_chunk M64))) xm ?ss'" 
+        using c0_6 c0_3 a1 by argo 
+
+
+      have "fix_bpf_sem 2 (l_bin0,l_pc,l_jump) xst = fix_bpf_sem 1 (l_bin0,l_pc,l_jump) (fix_bpf_one_step (l_bin0,l_pc,l_jump) xst)"
+        by (metis Suc_1 fix_bpf_sem.simps(2)) 
+      hence d0:"fix_bpf_sem 2 (l_bin0,l_pc,l_jump) xst = fix_bpf_sem 1 (l_bin0,l_pc,l_jump) (exec_instr Pret_anchor sz xpc xrs xm xss)"
+        using b2_0 a3 b2 by(unfold fix_bpf_one_step_def Let_def,simp_all)
+      hence d1:"fix_bpf_sem 2 (l_bin0,l_pc,l_jump) xst = fix_bpf_sem 1 (l_bin0,l_pc,l_jump) (exec_ret_external xpc sz M64 xm xss xrs)" using exec_instr_def by simp
+      have d2:" (\<exists> xpc1 xrs1 xm1 xss1. exec_ret_external xpc sz M64 xm xss xrs = Next xpc1 xrs1 xm1 xss1 \<and>
+        (let (pc', ss', caller,fp) = update_stack2 xss in 
+          let rs' = restore_x64_caller xrs caller fp in ss' = xss1 \<and> xm1 = xm \<and> xpc1 = xpc + sz \<and> xrs1 = rs'))"
+        using exec_ret_external_prop by blast
+
+      then obtain xpc1 xrs1 xm1 xss1 where d3:"exec_ret_external xpc sz M64 xm xss xrs = Next xpc1 xrs1 xm1 xss1 \<and>
+        (let (pc', ss', caller,fp) = update_stack2 xss in 
+          let rs' = restore_x64_caller xrs caller fp in ss' = xss1 \<and> xm1 = xm \<and> xpc1 = xpc+sz \<and> xrs1 = rs')" by auto
+
+      hence d3_0:"Next xpc1 xrs1 xm1 xss1 = Next (xpc+sz) (restore_x64_caller xrs (fst(snd(snd(update_stack2 xss)))) (snd(snd(snd(update_stack2 xss))))) xm (fst(snd(update_stack2 xss)))" 
+              apply(unfold Let_def,simp_all)
+        by(cases "update_stack2 xss",simp_all)
+
+      hence d4:"fix_bpf_sem 2 (l_bin0,l_pc,l_jump) xst = fix_bpf_sem 1 (l_bin0,l_pc,l_jump) (Next xpc1 xrs1 xm1 xss1)" using d1 d3 by argo 
+
+      hence d4_0:"xpc1 = (xpc+sz) \<and> xm = xm1 \<and> xrs1 = ?rs' \<and> xss1 = ?ss'" 
+        using d4 d3_0 by fastforce
+
+      let "?pc" = "fst (update_stack2 xss)"
+      have e0:"find_target_pc_in_l_pc3 l_jump (uint pc) = Some (uint ?pc)" using cn by simp
+
+      have "fix_bpf_sem 1 (l_bin0,l_pc,l_jump) (Next xpc1 xrs1 xm1 xss1) = fix_bpf_one_step (l_bin0,l_pc,l_jump) (Next xpc1 xrs1 xm1 xss1)" by fastforce
+      hence d5:"fix_bpf_sem 1 (l_bin0,l_pc,l_jump) (Next xpc1 xrs1 xm1 xss1) =  (exec_instr Pret sz xpc1 xrs1 xm1 xss1)" 
+        using b2_2 d4_0 apply(unfold fix_bpf_one_step_def,simp_all) by (simp add: exec_instr_def) 
+
+      have e1:"find_target_pc_in_l_pc2 l_pc (int xpc1) 0 = Some (uint pc)" using l_pc_index_corr sorry
+
+      hence "exec_instr Pret sz2 xpc1 xrs1 xm1 xss1 =  
+        (let nsp =  (xrs1 (IR SP)) + (u64_of_memory_chunk M64) in
+            case Mem.loadv M64 xm1 (Vptr sp_block nsp) of
+            None \<Rightarrow> Stuck |
+            Some ra \<Rightarrow> (
+              case ra of
+              Vlong v \<Rightarrow> let rs1 = xrs1#(IR SP) <- nsp in
+                          Next (unat v) rs1 xm1 xss1 |
+              _ \<Rightarrow> Stuck)
+        )" by(unfold exec_instr_def exec_ret_def,simp_all)
+
+      hence "exec_instr Pret sz2 xpc1 xrs1 xm1 xss1 = Next (unat v) (?rs'#(IR SP) <- ((?rs' (IR SP)) + (u64_of_memory_chunk M64))) xm1 xss1"
+        using d4_0 c0_5
+        using c0_7 by presburger 
+      hence "fix_bpf_sem 2 (l_bin0,l_pc,l_jump) xst = snd fxst'"
+        using d4 d5 c1 apply (simp add: exec_instr_def) using d4_0 by fastforce 
+      hence "\<exists> num fst'. fix_bpf_sem num (l_bin0,l_pc,l_jump) xst = fst' \<and> match_state2 fst' (snd fxst')"
+        using c1 match_state2_def match_mem_def
+        by (smt (verit, del_insts) outcome.simps(4)) 
+      then show ?thesis by blast
+    next
+      case False
+      have "\<not> (\<exists> sz src dst. x64_decode xpc l_bin0 = Some(sz, Pcmpq_rr src dst)) \<and> \<not> (\<exists> sz imm. x64_decode xpc l_bin0 = Some(sz, Pcall_i imm)) \<and> \<not>(\<exists> sz. x64_decode xpc l_bin0 = Some(sz, Pret_anchor))" using b2 False by simp
+      hence c0:"snd fxst' = (let num = snd (l_pc!(unat pc)) in x64_sem num l_bin0 (Next xpc xrs xm xss))"
+        using b0_1 b0_2 b0_3 a3 apply(unfold flat_bpf_one_step_def Let_def,simp_all)apply(cases "x64_decode xpc l_bin0",simp_all)
+        subgoal for a apply(cases a,simp_all)
+          subgoal for aa b apply(cases b,simp_all)
+            done
+          done
+        done
+      let "?num" = "snd (l_pc!(unat pc))"
+      have cn:"x64_bin_is_sequential ?num l_bin0 xpc" by (meson False a4 a2 a5 b2 x64_bin_is_sequential_x64_decode3) 
+
+      have d0:"x64_sem ?num l_bin0 (Next xpc xrs xm xss) = fix_bpf_sem ?num (l_bin0,l_pc,l_jump) xst" 
+        using x64_bin_is_sequential_equivalence a3 cn by presburger 
+      then show ?thesis
+         using c0 by (smt (verit, best) a1 match_mem_def match_state2_def outcome.simps(4)) 
+    qed
+  qed
+ qed
+qed
+
+
+
+end
