theory/JITFix_def.thy
@@ -1,0 +1,208 @@
+theory JITFix_def
+imports JITFlattern
+begin
+
+fun find_target_pc_in_l_pc2 :: "((int\<times>nat) list) \<Rightarrow> int \<Rightarrow> int \<Rightarrow> int option" where
+"find_target_pc_in_l_pc2 [] _ _ = None" |
+"find_target_pc_in_l_pc2 (x#xs) xpc num = (
+  if fst x = xpc then Some num
+  else find_target_pc_in_l_pc2 xs xpc (num+1)
+)"
+
+
+fun find_num_in_l_pc :: "((int\<times>nat) list) \<Rightarrow> int \<Rightarrow> nat option" where
+"find_num_in_l_pc [] _ = None" |
+"find_num_in_l_pc ((x,y)#xs) xpc = (
+  if x = xpc then Some y
+  else find_num_in_l_pc xs xpc 
+)"
+
+
+value "find_target_pc_in_l_pc2 [(0,1),(1,2),(3,3)] 3 0"
+
+value "find_num_in_l_pc [(0,1),(1,2),(3,3)] 3"
+
+(*definition flat_bpf_one_step :: "flat_bpf_prog \<Rightarrow> outcome \<Rightarrow> outcome" where
+"flat_bpf_one_step lp xst = (
+  let (l_bin,l_pc,l_jump) = lp in  
+    (case xst of
+    Stuck \<Rightarrow> Stuck |
+    Next xpc rs m ss \<Rightarrow> (
+    let v = find_target_pc_in_l_pc2 l_pc (int xpc) 0 ; v2 = find_num_in_l_pc l_pc (int xpc) in 
+      case v of None \<Rightarrow> Stuck | Some pc \<Rightarrow>
+        (case v2 of None \<Rightarrow> Stuck | Some num \<Rightarrow>
+          (case x64_decode xpc l_bin of Some(sz, Pcall_i d) \<Rightarrow>
+            (case find_target_pc_in_l_pc l_jump pc of 
+              None \<Rightarrow> Stuck |
+              Some npc \<Rightarrow> 
+                (let caller = save_x64_caller rs; fp = save_x64_frame_pointer rs; 
+                    rs' = upate_x64_stack_pointer rs (stack_pointer ss) in
+                let ss' = update_stack caller fp (of_int pc+1) ss in
+                  (case ss' of None \<Rightarrow> Stuck | 
+                  Some ra \<Rightarrow> (Next (nat (fst (l_pc!(unat npc)))) rs' m ra))))  |
+              Some(_,Pret) \<Rightarrow>
+                  let (pc', ss', caller,fp) = update_stack2 ss in 
+                  let rs' = restore_x64_caller rs caller fp in Next (nat(fst(l_pc!(unat pc')))) rs' m ss' |
+    _ \<Rightarrow> (x64_sem num l_bin (Next xpc rs m ss))
+       
+)))))"*)
+
+(*
+definition fix_bpf_one_step :: "flat_bpf_prog \<Rightarrow> outcome \<Rightarrow> outcome" where
+"fix_bpf_one_step lp xst = (
+  let (l_bin,l_pc,l_jump) = lp in  
+    (case xst of
+    Stuck \<Rightarrow> Stuck |
+    Next xpc rs m ss \<Rightarrow> (
+    let v = find_target_pc_in_l_pc2 l_pc (int xpc) 0 ; v2 = find_num_in_l_pc l_pc (int xpc) in 
+      case v of None \<Rightarrow> Stuck | Some pc \<Rightarrow>
+        (case v2 of None \<Rightarrow> Stuck | Some num \<Rightarrow>
+          (case x64_decode xpc l_bin of Some(sz, Pcall_i d) \<Rightarrow>
+            (case find_target_pc_in_l_pc l_jump pc of 
+              None \<Rightarrow> Stuck |
+              Some npc \<Rightarrow> 
+                (let caller = save_x64_caller rs; fp = save_x64_frame_pointer rs; 
+                    rs' = upate_x64_stack_pointer rs (stack_pointer ss) in
+                let ss' = update_stack caller fp (of_nat xpc) ss in
+                  (case ss' of None \<Rightarrow> Stuck | 
+                  Some ra \<Rightarrow> (Next (nat (fst (l_pc!(unat npc)))) rs' m ra))))  |
+                  Some(_, Pcmpq_rr src dst) \<Rightarrow> \<comment>\<open> TODO: if the first byte is the opcode of cmp? \<close>
+                          \<comment>\<open> case: BPF JMP \<close>
+                          (case x64_sem num l_bin (Next xpc rs m ss) of
+                          Stuck \<Rightarrow> Stuck | \<comment>\<open> if one step error, stop, it should be impossible \<close>
+                          Next xpc1 rs1 m1 ss1 \<Rightarrow> (
+                            if rs1 (CR ZF) = 1 then \<comment>\<open> must JUMP \<close>
+                              (case find_target_pc_in_l_pc l_jump pc of
+                              None \<Rightarrow> Stuck |
+                              Some npc \<Rightarrow>
+                                (Next (nat (fst (l_pc!(unat npc)))) rs1 m1 ss1)) \<comment>\<open> go to the target address in the jited x64 binary \<close>
+                            else \<comment>\<open> donot JUMP \<close>
+                              (Next xpc1 rs1 m1 ss1)
+                          )) |
+              Some(_,Pret) \<Rightarrow>
+                  let (xpc', ss', caller,fp) = update_stack2 ss in 
+                  let rs' = restore_x64_caller rs caller fp in Next (unat xpc') rs' m ss' |
+    _ \<Rightarrow> (x64_sem num l_bin (Next xpc rs m ss))
+       
+)))))"
+*)
+
+(*
+definition fix_bpf_one_step :: "flat_bpf_prog \<Rightarrow> outcome \<Rightarrow> outcome" where
+"fix_bpf_one_step lp xst = (
+  let (l_bin,l_pc,l_jump) = lp in  
+    (case xst of
+    Stuck \<Rightarrow> Stuck |
+    Next xpc rs m ss \<Rightarrow> (
+          (case x64_decode xpc l_bin of 
+                  Some(sz, Pcall_i imm) \<Rightarrow>
+                      let v = find_target_pc_in_l_pc2 l_pc (int xpc) 0 in
+                      (case v of None \<Rightarrow> Stuck | Some pc \<Rightarrow>
+                      (case find_target_pc_in_l_pc l_jump pc of
+                        None \<Rightarrow> Stuck |
+                        Some npc \<Rightarrow>
+                      exec_instr (Pcall_i (of_int(fst (l_pc!(unat npc))))) sz xpc rs m ss)) |
+                  Some(sz, Pjcc cond d) \<Rightarrow> 
+                      let v = find_target_pc_in_l_pc2 l_pc (int xpc-3) 0 in
+                      (case v of None \<Rightarrow> Stuck | Some pc \<Rightarrow>
+                      (case find_target_pc_in_l_pc l_jump pc of
+                        None \<Rightarrow> Stuck |
+                        Some npc \<Rightarrow>
+                          (exec_instr (Pjcc cond (of_int (fst (l_pc!(unat npc)))-(of_nat (xpc+1)))) sz xpc rs m ss))) |
+                  Some(sz, Pret) \<Rightarrow> 
+                      let v = find_target_pc_in_l_pc2 l_pc (int xpc) 0 in
+                      (case v of None \<Rightarrow> Stuck | Some pc \<Rightarrow>
+                      (case (exec_instr Pret sz xpc rs m ss) of Stuck \<Rightarrow> Stuck | 
+                                          Next xpc1 rs1 m1 ss1 \<Rightarrow> let v2 = find_target_pc_in_l_pc3 l_jump pc in
+                                            (case v2 of None \<Rightarrow> Stuck | Some pc'\<Rightarrow>
+                                              (if xpc1 \<noteq> nat (fst (l_pc!(nat pc')))+1 then Stuck else Next xpc1 rs1 m1 ss1 )))) |
+                  Some(sz,ins) \<Rightarrow> (exec_instr ins sz xpc rs m ss) |
+                  _ \<Rightarrow> Stuck 
+))))"*)
+
+
+(*
+definition fix_bpf_one_step :: "flat_bpf_prog \<Rightarrow> outcome \<Rightarrow> outcome" where
+"fix_bpf_one_step lp xst = (
+  let (l_bin,l_pc,l_jump) = lp in  
+    (case xst of
+    Stuck \<Rightarrow> Stuck |
+    Next xpc rs m ss \<Rightarrow> (
+          (case x64_decode xpc l_bin of 
+                  Some(sz, Pcall_i imm) \<Rightarrow>
+                      let v = find_target_pc_in_l_pc2 l_pc (int xpc) 0 in
+                      (case v of None \<Rightarrow> Stuck | Some pc \<Rightarrow>
+                      (case find_target_pc_in_l_pc l_jump pc of
+                        None \<Rightarrow> Stuck |
+                        Some npc \<Rightarrow>
+                      exec_instr (Pcall_i (of_int(fst (l_pc!(unat npc))))) sz xpc rs m ss)) |
+                  Some(sz, Pjcc cond d) \<Rightarrow> 
+                      let v = find_target_pc_in_l_pc2 l_pc (int xpc-3) 0 in
+                      (case v of None \<Rightarrow> Stuck | Some pc \<Rightarrow>
+                      (case find_target_pc_in_l_pc l_jump pc of
+                        None \<Rightarrow> Stuck |
+                        Some npc \<Rightarrow>
+                          (exec_instr (Pjcc cond (of_int (fst (l_pc!(unat npc)))-(of_nat (xpc+1)))) sz xpc rs m ss))) |
+                  Some(sz, Pret) \<Rightarrow> 
+                      let v = find_target_pc_in_l_pc2 l_pc (int xpc) 0 in
+                      (case v of None \<Rightarrow> Stuck | Some pc \<Rightarrow>
+                      (case (exec_instr Pret sz xpc rs m ss) of Stuck \<Rightarrow> Stuck | 
+                                          Next xpc1 rs1 m1 ss1 \<Rightarrow> let v2 = find_target_pc_in_l_pc3 l_jump pc in
+                                            (case v2 of None \<Rightarrow> Stuck | Some pc'\<Rightarrow>
+                                              (if xpc1 \<noteq> nat (fst (l_pc!(nat pc')))+1 then Stuck else Next xpc1 rs1 m1 ss1 )))) |
+                  Some(sz,ins) \<Rightarrow> (exec_instr ins sz xpc rs m ss) |
+                  _ \<Rightarrow> Stuck 
+))))"
+*)
+
+definition fix_bpf_one_step :: "flat_bpf_prog \<Rightarrow> outcome \<Rightarrow> outcome" where
+"fix_bpf_one_step lp xst = (
+  let (l_bin,l_pc,l_jump) = lp in  
+    (case xst of
+    Stuck \<Rightarrow> Stuck |
+    Next xpc rs m ss \<Rightarrow> (
+          (case x64_decode xpc l_bin of 
+                  Some(sz, Pcall_i imm) \<Rightarrow>
+                      let v = find_target_pc_in_l_pc2 l_pc (int xpc) 0 in
+                      (case v of None \<Rightarrow> Stuck | Some pc \<Rightarrow>
+                      (case find_target_pc_in_l_pc l_jump pc of
+                        None \<Rightarrow> Stuck |
+                        Some npc \<Rightarrow>
+                      exec_instr (Pcall_i (of_int(fst (l_pc!(unat npc))))) sz xpc rs m ss)) |
+                  Some(sz, Pjcc cond d) \<Rightarrow> 
+                      let v = find_target_pc_in_l_pc2 l_pc (int xpc-3) 0 in
+                      (case v of None \<Rightarrow> Stuck | Some pc \<Rightarrow>
+                      (case find_target_pc_in_l_pc l_jump pc of
+                        None \<Rightarrow> Stuck |
+                        Some npc \<Rightarrow>
+                          (exec_instr (Pjcc cond (of_int (fst (l_pc!(unat npc)))-(of_nat (xpc+1)))) sz xpc rs m ss))) |
+                  Some(sz,ins) \<Rightarrow> (exec_instr ins sz xpc rs m ss) |
+                  _ \<Rightarrow> Stuck 
+))))"
+
+
+
+
+fun fix_bpf_sem :: "nat \<Rightarrow> flat_bpf_prog \<Rightarrow> outcome \<Rightarrow> outcome" where
+"fix_bpf_sem 0 _ xst = xst" |
+"fix_bpf_sem (Suc n) lt xst = (
+   let pair = fix_bpf_one_step lt xst in
+    fix_bpf_sem n lt pair
+)"
+
+(*
+definition match_state2::"outcome \<Rightarrow> outcome \<Rightarrow> bool" where
+  "match_state2 fxst xxst \<equiv> 
+  fxst = xxst \<and> (fxst \<noteq> Stuck \<or> xxst \<noteq> Stuck)"
+*)
+
+definition match_state2::"outcome \<Rightarrow> outcome \<Rightarrow> bool" where
+  "match_state2 fxst xxst \<equiv> 
+  (case fxst of (Next xpc xrs xm xss) \<Rightarrow>
+    (case xxst of (Next xpc1 xrs1 xm1 xss1) \<Rightarrow> 
+    xpc = xpc1 \<and> xrs = xrs1 \<and> match_mem xm xm1 \<and> xss = xss1 |
+                   _ \<Rightarrow> False)|
+                 _ \<Rightarrow> False)"
+
+
+end
