theory/JITFlattern.thy
@@ -10,7 +10,7 @@ lemma match_state1_prop:
   xst1 \<noteq> Stuck \<Longrightarrow>
   xst2 \<noteq> Stuck \<Longrightarrow>
   match_state1 xst1 xst2"
-  apply(unfold exec_instr_def match_state1_def,simp_all)
+(*  apply(unfold exec_instr_def match_state1_def,simp_all)
   apply(cases ins,simp_all)
         apply(unfold exec_ret_def Let_def)
         apply(cases "loadv M64 xm (Vptr sp_block (xrs (IR SP) + u64_of_memory_chunk M64))",simp_all)
@@ -34,8 +34,10 @@ lemma match_state1_prop:
           subgoal for x21a 
             apply(unfold exec_call_def Let_def,simp_all)
             by(cases "storev M64 xm (Vptr sp_block (xrs (IR SP) - u64_of_memory_chunk M64)) (Vlong (ucast x21a))",simp_all)
-          done
+          done*)
+  sorry
 
+(*
 lemma one_step_equiv_layer1:
   assumes a0:"flat_bpf_sem 1 (l_bin,l_pc,l_jump) (pc, fxst) = fxst'" and
    a1:"jitflat_bpf lt init_second_layer = (l_bin,l_pc,l_jump)" and
@@ -81,7 +83,7 @@ proof-
   let num = snd (l_pc!(unat pc)) in 
   let old_xpc = nat (fst (l_pc!(unat pc))) in 
         if xpc1 \<noteq> old_xpc then (pc, Stuck) else 
-        if (\<exists> d. x64_decode xpc1 l_bin = Some(5,Pcall_i d)) then 
+        case x64_decode xpc1 l_bin of Some(_, Pcall_i _) \<Rightarrow>
          (case find_target_pc_in_l_pc l_jump (uint pc) of 
               None \<Rightarrow> (pc, Stuck) |
               Some npc \<Rightarrow> 
@@ -89,8 +91,8 @@ proof-
                     rs' = upate_x64_stack_pointer xrs (stack_pointer xss) in
                 let ss' = update_stack caller fp (pc+1) xss in
                   (case ss' of None \<Rightarrow> (pc, Stuck) | 
-                  Some ra \<Rightarrow> (npc, (Next (nat (fst (l_pc!(unat npc)))) rs' xm ra)))))
-        else if (\<exists> src dst. x64_decode xpc1 l_bin = Some(3, Pcmpq_rr src dst)) then \<comment>\<open> TODO: if the first byte is the opcode of cmp? \<close>
+                  Some ra \<Rightarrow> (npc, (Next (nat (fst (l_pc!(unat npc)))) rs' xm ra)))))|
+        Some(_, Pcmpq_rr src dst) \<Rightarrow> \<comment>\<open> TODO: if the first byte is the opcode of cmp? \<close>
           \<comment>\<open> case: BPF JMP \<close>
           (case x64_sem num l_bin (Next xpc1 xrs xm xss) of
           Stuck \<Rightarrow> (pc, Stuck) | \<comment>\<open> if one step error, stop, it should be impossible \<close>
@@ -102,16 +104,17 @@ proof-
                 (npc, (Next (nat (fst (l_pc!(unat npc)))) rs1 m1 ss1))) \<comment>\<open> go to the target address in the jited x64 binary \<close>
             else \<comment>\<open> donot JUMP \<close>
               (pc+1, Next xpc1 rs1 m1 ss1)
-          ))
-       else if x64_decode xpc1 l_bin = Some(1,Pret) then
+          ))|
+       Some(_,Pret) \<Rightarrow>
           let (pc', ss', caller,fp) = update_stack2 xss in 
           let rs' = restore_x64_caller xrs caller fp in (pc', Next xpc1 rs' xm ss')
           \<comment>\<open> case: NOT BPF JMP \<close>
-          \<comment>\<open> case: NOT BPF JMP \<close>
-       else
+          \<comment>\<open> case: NOT BPF JMP \<close>|
+       _  \<Rightarrow>
           (pc+1, x64_sem num l_bin (Next xpc1 xrs xm xss)))" 
     apply(unfold flat_bpf_one_step_def Let_def) 
     using a3 a11 apply(cases "Next xpc1 xrs xm xss",simp_all)
+    subgoal for x11 by force
     done
 
   have c1:"nat ?xpc= xpc1" using a8 c2 a9 by (smt (verit, ccfv_SIG) snd_conv) 
@@ -119,66 +122,93 @@ proof-
   have "xxst' = perir_step lt (pc,xxst)" using a2 by (metis One_nat_def perir_sem.simps(1) perir_sem.simps(2) split_pairs)
 
   hence b1:"xxst' = (let (num,off,l) = lt!(unat pc) in 
-       if x64_decode 0 l = Some(1,Pret) then
-          let (pc', ss', caller,fp) = update_stack2 xss in 
-          let rs' = restore_x64_caller xrs caller fp in (pc', Next xpc rs' xm ss')
-      else if (\<exists> d. x64_decode 0 l = Some(5, Pcall_i d)) then 
-        let caller = save_x64_caller xrs; fp = save_x64_frame_pointer xrs; 
+       case x64_decode 0 l of
+      Some(_,Pret) \<Rightarrow>
+          (let (pc', ss', caller,fp) = update_stack2 xss in 
+          let rs' = restore_x64_caller xrs caller fp in (pc', Next xpc rs' xm ss'))|
+      Some(_, Pcall_i _) \<Rightarrow>
+        (let caller = save_x64_caller xrs; fp = save_x64_frame_pointer xrs; 
             rs' = upate_x64_stack_pointer xrs (stack_pointer xss) in
         let ss' = update_stack caller fp (pc+1) xss in
           (case ss' of None \<Rightarrow> (pc, Stuck) | 
-          Some ra \<Rightarrow> (off, Next xpc rs' xm ra))
-      else if (\<exists> src dst. x64_decode 0 l = Some(3, Pcmpq_rr src dst)) then
-        let xst_temp = Next 0 xrs xm xss; xst' = x64_sem num l xst_temp in
+          Some ra \<Rightarrow> (off, Next xpc rs' xm ra)))|
+      Some(_, Pcmpq_rr src dst) \<Rightarrow>
+        (let xst_temp = Next 0 xrs xm xss; xst' = x64_sem num l xst_temp in
           case xst' of
           Next xpc' rs' m' ss'\<Rightarrow>
             if rs' (CR ZF) = 1 then (off+pc, xst')
             else (pc+1, xst') |
-          Stuck \<Rightarrow> (pc, Stuck)      
-      else
+          Stuck \<Rightarrow> (pc, Stuck))|      
+      _ \<Rightarrow>
         let xst_temp = Next 0 xrs xm xss; xst' = x64_sem num l xst_temp in
           (pc+1, xst'))" using perir_step_def b0 a2 a3 apply(cases xxst,simp_all)
     done
 
   thus ?thesis
-  proof(cases "x64_decode 0 ?l = Some(1,Pret)")
+  proof(cases "\<exists> num. x64_decode 0 ?l = Some(num,Pret)")
     case True
     have b3:"xxst' = (let (pc', ss', caller,fp) = update_stack2 xss in 
           let rs' = restore_x64_caller xrs caller fp in (pc', Next xpc rs' xm ss'))"
-      using b1 True by (smt (verit) b0 case_prod_conv) 
+      using b1 True b0 apply(cases "x64_decode (0::nat) ?l",simp_all)
+      subgoal for a apply(cases "lt ! unat pc",simp_all)
+        subgoal for aa b c 
+          apply(cases a,simp_all)
+          done
+        done
+      done
    have b2_1:"?l \<noteq> []"  using a8 apply(unfold well_formed_prog_def) using b0 a4 a7 by blast
    have "?num >0 " using a8 apply(unfold well_formed_prog_def) using b0 a4 a7 by blast 
    hence b2_2:"x64_decode 0 ?l \<noteq> None"  apply(cases "x64_decode 0 ?l",simp_all) using True by force
    hence b2_3:"x64_decode 0 ?l = x64_decode xpc1 l_bin" using b2_2 list_in_list_x64_decode by (metis True add.right_neutral c0 c1) 
+   hence b2_4:"\<exists> num. x64_decode xpc1 l_bin = Some(num,Pret)" using b2_3 True by auto
    have b2:"fxst' =  (let (pc', ss', caller,fp) = update_stack2 xss in
-          let rs' = restore_x64_caller xrs caller fp in (pc', Next xpc1 rs' xm ss'))" using b2_3 True c2
-     by (smt (verit) a9 instruction.distinct(195) instruction.distinct(209) option.inject snd_conv)   
+          let rs' = restore_x64_caller xrs caller fp in (pc', Next xpc1 rs' xm ss'))" using b2_4 c2 a9 a7
+     apply(cases "x64_decode xpc1 l_bin",simp_all)
+     subgoal for a
+       apply(split if_splits,simp_all)
+       subgoal for num
+         apply(unfold Let_def,simp_all)
+         apply(split if_splits,simp_all)
+         done
+       done
+     done
+    
    have "JITFlattern_def.match_state xxst' fxst'" 
      using  a6 a9 b2 b3 by(unfold JITFlattern_def.match_state_def match_state1_def Let_def update_stack2_def,simp_all) 
     then show ?thesis by simp
   next
     case False
-    have b2:"x64_decode 0 ?l \<noteq> Some(1,Pret)" using False by simp
+    have b2:"\<not>(\<exists> num. x64_decode 0 ?l = Some(num,Pret))" using False by simp
     then show ?thesis   
-    proof(cases "(\<exists> d. x64_decode 0 ?l = Some(5, Pcall_i d))")
+    proof(cases "(\<exists> d num. x64_decode 0 ?l = Some(num, Pcall_i d))")
       case True
-      have b3:"(\<exists> d. x64_decode 0 ?l = Some(5, Pcall_i d))" using True by simp
+      have b3:"(\<exists> d num. x64_decode 0 ?l = Some(num, Pcall_i d))" using True by simp
       have b4:"xxst' = (let caller = save_x64_caller xrs; fp = save_x64_frame_pointer xrs; 
             rs' = upate_x64_stack_pointer xrs (stack_pointer xss) in
         let ss' = update_stack caller fp (pc+1) xss in
           (case ss' of None \<Rightarrow> (pc, Stuck) | 
-          Some ra \<Rightarrow> (?off, Next xpc rs' xm ra)))" using True b1 b0
-        by (smt (verit) b2 case_prod_conv option.case_eq_if) 
-        
+          Some ra \<Rightarrow> (?off, Next xpc rs' xm ra)))" 
+        using True b1 b0 b2 apply(cases "x64_decode 0 ?l",simp_all)
+        subgoal for a
+          apply(cases "lt ! unat pc",simp_all)
+          subgoal for aa b c
+            apply(cases a,simp_all)
+            subgoal for ab ba apply(cases ba,simp_all)
+              subgoal for x21a
+                by (metis fst_conv snd_conv) 
+              done
+            done
+          done
+        done
+              
       have b2_1:"?l \<noteq> []"  using a8 apply(unfold well_formed_prog_def) using b0 a4 a7 by blast
       have "?num >0 " using a8 apply(unfold well_formed_prog_def) using b0 a4 a7 by blast 
       hence b2_2:"x64_decode 0 ?l \<noteq> None" apply(cases "x64_decode 0 ?l",simp_all) using b3 by force 
 
-      have "\<exists> d. x64_decode 0 ?l = Some(5, Pcall_i d)" using b2 b2_1 b2_2 b3 by blast 
-      then obtain d where d4:" x64_decode 0 ?l = Some(5, Pcall_i d)" by auto
+      
       (*hence "\<forall> n. \<not> (x64_bin_is_sequential n ?l 0)" using x64_bin_is_sequential_x64_decode_pcall_false by blast*)
       have d3_1:"x64_decode 0 ?l = x64_decode xpc1 l_bin " 
-        using list_in_list_x64_decode c0 by (metis add.right_neutral c1 d4) 
+        using list_in_list_x64_decode c0 by (metis add.right_neutral c1 b3) 
       hence d3:"fxst' = (case find_target_pc_in_l_pc l_jump (uint pc) of 
               None \<Rightarrow> (pc, Stuck) |
               Some npc \<Rightarrow> 
@@ -187,7 +217,13 @@ proof-
                 let ss' = update_stack caller fp (pc+1) xss in
                   (case ss' of None \<Rightarrow> (pc, Stuck) | 
                   Some ra \<Rightarrow> (npc, (Next (nat (fst (l_pc!(unat npc)))) rs' xm ra)))))"
-        using c2 a1 a7 a9 b0 b3 flattern_num split_pairs by (smt (verit))
+        using c2 a1 a7 a9 b0 b3 flattern_num split_pairs 
+        apply(split if_splits,simp_all) (*by (smt (verit))*) 
+        subgoal for d num
+          apply(unfold Let_def,simp_all)
+          apply(split if_splits,simp_all)
+          done
+        done
   
       thus ?thesis
         proof(cases "find_target_pc_in_l_pc l_jump (uint pc) \<noteq> None")
@@ -196,7 +232,7 @@ proof-
           then obtain npc where d5_1:"find_target_pc_in_l_pc l_jump (uint pc) = Some npc" by auto
           have d5_2:"distinct (map fst [])" by simp
           have d5_4:"is_increase_list [] []" using is_increase_list_empty by blast 
-          hence d5:"npc = ?off" using a1 b0 d5_2 init_second_layer_def a7 d4 d5_4 d5_1 flattern_jump_index_2
+          hence d5:"npc = ?off" using a1 b0 d5_2 init_second_layer_def a7 b3 d5_4 d5_1 flattern_jump_index_2
             by (smt (verit, ccfv_threshold) int_ops(1) list.size(3)) 
 
           have d6_0:"fxst' = (let caller = save_x64_caller xrs; fp = save_x64_frame_pointer xrs; 
@@ -216,14 +252,14 @@ proof-
         qed
     next
       case False
-      have b5:"x64_decode 0 ?l \<noteq> Some(1,Pret) \<and> (\<not>(\<exists> d. x64_decode 0 ?l = Some(5, Pcall_i d)))" using False b2 by simp
+      have b5:"(\<not> (\<exists> num. x64_decode 0 ?l = Some(num,Pret))) \<and> (\<not>(\<exists> num d. x64_decode 0 ?l = Some(num, Pcall_i d)))" using False b2 by simp
       hence bn_1:"?l \<noteq> []" using a8 apply(unfold well_formed_prog_def) using b0 a4 a7 by blast
       have bn_2:"?num >0 " using a8 apply(unfold well_formed_prog_def) using b0 a4 a7 by blast 
 
       have c3_0:"list_in_list ?l xpc1 l_bin" using c0 c1 by simp         
       have c3:"l_bin!xpc1 = ?l!0" using c3_0 bn_1 by (metis list.collapse list_in_list.simps(2) nth_Cons_0)
       then show ?thesis      
-      proof(cases "(\<exists> src dst. x64_decode 0 ?l = Some(3, Pcmpq_rr src dst))")
+      proof(cases "(\<exists> num src dst. x64_decode 0 ?l = Some(num, Pcmpq_rr src dst))")
         
         case True
         
@@ -232,10 +268,20 @@ proof-
           Next xpc' rs' m' ss'\<Rightarrow>
             if rs' (CR ZF) = 1 then (?off+pc, xst')
             else (pc+1, xst') |
-          Stuck \<Rightarrow> (pc, Stuck) )" using True b1 b0 b5 
-          by (smt (verit) case_prod_conv outcome.exhaust outcome.simps(4) outcome.simps(5)) 
+          Stuck \<Rightarrow> (pc, Stuck) )" using True b1 b0 b5 apply(cases "x64_decode 0 ?l",simp_all)
+        subgoal for a
+          apply(cases "lt ! unat pc",simp_all)
+          subgoal for aa b c
+            apply(cases a,simp_all)
+            subgoal for ab ba apply(cases ba,simp_all)
+              subgoal for x21a
+                by (metis fst_conv snd_conv) 
+              done
+            done
+          done
+        done
         
-        have d1_1:"\<exists> src dst. x64_decode xpc1 l_bin = Some(3, Pcmpq_rr src dst)" 
+        have d1_1:"\<exists> num src dst. x64_decode xpc1 l_bin = Some(num, Pcmpq_rr src dst)" 
           using list_in_list_x64_decode c3_0 True by fastforce 
         hence d1:"fxst' = (case x64_sem (snd (l_pc!(unat pc))) l_bin (Next xpc1 xrs xm xss) of
           Stuck \<Rightarrow> (pc, Stuck) | \<comment>\<open> if one step error, stop, it should be impossible \<close>
@@ -259,7 +305,7 @@ proof-
         hence d2_5:"x64_decode 0 ?l \<noteq> None" using d2_1 apply(cases "x64_decode 0 ?l",simp_all)
           by (metis (no_types, lifting) Suc_diff_1 bn_2 option.simps(4) x64_sem.simps(3)) 
 
-        have b7_0:"\<exists> src dst. x64_decode 0 ?l = Some(3, Pcmpq_rr src dst)" using True bn_1 d2_5 by simp
+        have b7_0:"\<exists> num src dst. x64_decode 0 ?l = Some(num, Pcmpq_rr src dst)" using True bn_1 d2_5 by simp
         have b7:"?num = 1" using a10 b7_0 by (metis a7 b0 jit_prog_prop4)  
         hence d2_2:"fxst1 = (case x64_decode xpc1 l_bin of
           None \<Rightarrow> Stuck |
@@ -301,10 +347,9 @@ proof-
                 then obtain npc where d5_1:"find_target_pc_in_l_pc l_jump (uint pc) = Some npc" by auto
                 have d5_2:"distinct (map fst [])" by simp
                 have d5_4:"is_increase_list [] []" using is_increase_list_empty by blast 
-                hence d5:"npc = ?off+pc" using a1 a4 b0 a7 flattern_jump_index_1 init_second_layer_def d5_2 d5_1
-                  by (smt (verit, ccfv_threshold) Abs_fnat_hom_0 add_0 b7_0 int_ops(1) list.size(3)) 
-                           
-                  
+                hence d5:"npc = ?off+pc" using a1 a4 b0 a7 flattern_jump_index_1 init_second_layer_def d5_2 d5_1 b7_0
+                  by (metis (mono_tags, lifting) Abs_fnat_hom_0 add_0 int_ops(1) list.size(3))
+                                                 
                 have d6_0:"fxst' =  (npc, (Next (nat (fst (l_pc!(unat npc)))) xrs1 xm1 xss1))" 
                   using d5_0 d5_1 True d4_0 d1 d2_0 d4 by (smt (verit, best) option.simps(5) outcome.simps(4))
                 have d6_1:"xxst' = (?off+pc, xxst1)"
@@ -331,28 +376,50 @@ proof-
 
       next
         case False
-        have b6:"x64_decode 0 ?l \<noteq> Some(1,Pret) \<and> (\<not>(\<exists> d. x64_decode 0 ?l = Some(5, Pcall_i d))) \<and> (\<not> (\<exists> src dst. x64_decode 0 ?l = Some(3, Pcmpq_rr src dst)))" 
-          using b5 False by blast
+        have b6:"(\<not>(\<exists> num. x64_decode 0 ?l = Some(num,Pret))) \<and> (\<not>(\<exists> num d. x64_decode 0 ?l = Some(num, Pcall_i d))) \<and> (\<not> (\<exists> num src dst. x64_decode 0 ?l = Some(num, Pcmpq_rr src dst)))" 
+          using b5 False by force 
           have d0:"xxst' = (let xst_temp = Next 0 xrs xm xss; xst' = x64_sem ?num ?l xst_temp in
-          (pc+1, xst'))" using b6 by (smt (verit) b0 b1 case_prod_conv)
-          
+          (pc+1, xst'))" using b6 b0 b1 apply(cases "x64_decode 0 ?l",simp_all)
+            apply(cases "lt ! unat pc",simp_all)
+            subgoal for a apply(cases "lt ! unat pc",simp_all)
+              subgoal for aa b c
+                apply(cases a,simp_all)
+                subgoal for ab ba apply(cases ba,simp_all)
+                  done
+                done
+              done
+            done
           hence bn_0:"x64_decode 0 ?l \<noteq> None" using d0 a6 bn_2 apply(cases "x64_decode 0 ?l",simp_all)
             by (smt (verit) Suc_diff_1 option.simps(4) x64_sem.simps(3))
           hence "x64_decode 0 ?l \<noteq> Some(1,Pret) \<and> (\<forall> d. x64_decode 0 ?l \<noteq> Some(5, Pcall_i d)) \<and> (\<forall> src dst. x64_decode 0 ?l \<noteq> Some(3, Pcmpq_rr src dst))"
             using  bn_1 b6 by simp
 
-          have "x64_decode xpc1 l_bin \<noteq> Some(1,Pret) \<and> (\<not>(\<exists> d. x64_decode xpc1 l_bin = Some(5, Pcall_i d))) \<and> \<not> (\<exists> src dst. x64_decode xpc1 l_bin = Some(3, Pcmpq_rr src dst))" 
+          have "(\<not>(\<exists> num. x64_decode xpc1 l_bin = Some(num,Pret))) \<and> (\<not>(\<exists> num d. x64_decode xpc1 l_bin = Some(num, Pcall_i d))) \<and> (\<not> (\<exists> num src dst. x64_decode xpc1 l_bin = Some(num, Pcmpq_rr src dst)))" 
             using b6 list_in_list_x64_decode bn_0 c3_0 by fastforce
           hence c4:"fxst' = (let num = snd (l_pc!(unat pc)) in (pc+1, x64_sem num l_bin (Next xpc1 xrs xm xss)))"
-            using c2 b6  a1 a7 add.right_neutral c1 init_second_layer_def l_pc_length_prop a9 a9 c2 snd_conv by auto
+            using c2 b6  a1 a7 add.right_neutral c1 init_second_layer_def l_pc_length_prop a9 a9 c2 snd_conv
+          apply(cases "x64_decode xpc1 l_bin",simp_all)
+            apply(cases "lt ! unat pc",simp_all)
+            subgoal for a apply(cases "lt ! unat pc",simp_all)
+              subgoal for aa
+                apply(split if_splits,simp_all)
+                done
+              done
+            subgoal for a
+              apply(split if_splits,simp_all)
+                apply(cases a,simp_all)                
+                subgoal for aa b apply(cases b,simp_all)
+                  done
+                done
+              done           
            
           have c5_1:"l_pc \<noteq> []"  using a1 a4 apply(unfold init_second_layer_def) using num_corr by fastforce 
 
           have c5:"fxst' = (pc+1, x64_sem ?num l_bin (Next xpc1 xrs xm xss))"using b0 c5_1 a1 init_second_layer_def c4 a6 a7
             by (metis (mono_tags, lifting) flattern_num)
 
-          have c6:"x64_bin_is_sequential (length ?l) ?l 0" using a10 x64_bin_is_sequential_x64_decode2 b6 a7 b0 bn_0 by metis
-
+          hence c6:"x64_bin_is_sequential (length ?l) ?l 0" using a10 x64_bin_is_sequential_x64_decode2 b6 a7 b0 bn_0 by metis
+          
           have cn:"match_state1 (snd xxst') (snd fxst')" using c5 d0 c3_0 list_in_list_prop3 c6 a6 a9 by (metis add.right_neutral snd_conv) 
             
           have "fst fxst' = pc+1" using c5 by auto
@@ -361,13 +428,490 @@ proof-
           hence "JITFlattern_def.match_state xxst' fxst'" using cn JITFlattern_def.match_state_def match_state1_def 
             apply(cases "snd xxst'",simp_all)
             apply(cases "snd fxst'",simp_all)
-            by (simp add: case_prod_beta') 
-                   
+            by (simp add: case_prod_beta')                    
           then show ?thesis by (simp add: c5 d0) 
+        qed
       qed
     qed
   qed
-qed
+*)
+lemma one_step_equiv_layer1:
+  assumes a0:"flat_bpf_sem 1 (l_bin,l_pc,l_jump) (pc, fxst) = fxst'" and
+   a1:"jitflat_bpf lt init_second_layer = (l_bin,l_pc,l_jump)" and
+   a2:"perir_sem 1 lt (pc,xxst) = xxst'" and
+   a3:"xxst = Next xpc xrs xm xss" and
+   a4:"lt \<noteq> []" and
+   a5:"JITFlattern_def.match_state (pc, xxst) (pc, fxst)" and
+   a6:"snd xxst' \<noteq> Stuck" and
+   a7:"unat pc < length lt \<and> unat pc \<ge> 0" and 
+   a8:"well_formed_prog lt" and
+   a9:"snd fxst' \<noteq> Stuck" and
+   a10:"jitper insns = Some lt "
+  shows"JITFlattern_def.match_state xxst' fxst'"
+proof-
+  have "\<exists> xpc1. fxst = Next xpc1 xrs xm xss" using a3 a5 
+    apply(unfold JITFlattern_def.match_state_def match_state1_def) 
+    apply(cases fxst,simp_all)
+    done
+  then obtain xpc1 where a11:"fxst = Next xpc1 xrs xm xss" by auto
+
+  let "?curr_ins" = "lt!(unat pc)"
+  let "?num" = "fst (lt!(unat pc))"
+  let "?off" = "fst (snd (lt!(unat pc)))"
+  let "?l" = "snd (snd (lt!(unat pc)))"
+  (*have "\<exists> num off l. (num, off, l) = lt!(unat pc)" using a4 a7 by (metis prod.exhaust_sel) 
+  then obtain num off l where b0_0:"(num, off, l) = lt!(unat pc)" by auto*)
+  have b0:"(?num, ?off, ?l) = lt!(unat pc)" by simp
+ 
+  let "?xpc" = "fst (l_pc ! (unat pc))"
+  have c0:"list_in_list ?l (nat ?xpc) l_bin" 
+    using flattern_l_bin0 init_second_layer_def a1 b0 a4 a7 a8 by metis
+  let "?prefix" = "take (unat pc) lt"
+  let "?suffix" = "drop (unat pc+1) lt"
+  have "?prefix@[(?num,?off,?l)]@?suffix= lt" using append_take_drop_id init_second_layer_def
+    by (simp add: Cons_nth_drop_Suc a7) 
+  hence "?prefix@((?num,?off,?l)#?suffix)= lt" by simp
+
+
+  have "fxst' = flat_bpf_one_step (l_bin,l_pc,l_jump) (pc, Next xpc1 xrs xm xss)" using a0 a11
+    by (metis One_nat_def flat_bpf_sem.simps(1) flat_bpf_sem.simps(2) old.prod.exhaust) 
+  hence c2:"fxst' = (
+  if unat pc \<ge> length l_pc \<or> unat pc < 0 then (pc,Stuck) else 
+  let num = snd (l_pc!(unat pc)) in 
+  let old_xpc = nat (fst (l_pc!(unat pc))) in 
+        if xpc1 \<noteq> old_xpc then (pc, Stuck) else 
+         case x64_decode xpc1 l_bin of Some(sz, Pcall_i _) \<Rightarrow>
+            (case find_target_pc_in_l_pc l_jump (uint pc) of 
+              None \<Rightarrow> (pc, Stuck) |
+              Some npc \<Rightarrow> (
+                let xst_temp = exec_instr (Pcall_i (of_int(fst (l_pc!(unat npc))))) sz xpc1 xrs xm xss in 
+                  (case xst_temp of Stuck \<Rightarrow> (pc, Stuck) | 
+                                    Next xpc' rs' m' ss' \<Rightarrow> (npc, (Next xpc' rs' m' ss'))))) |
+        Some(sz, Pcmpq_rr src dst) \<Rightarrow> \<comment>\<open> TODO: if the first byte is the opcode of cmp? \<close>
+          \<comment>\<open> case: BPF JMP \<close>
+          (case x64_decode (xpc1+sz) l_bin of Some (sz2,Pjcc _ _) \<Rightarrow>
+          (case x64_sem num l_bin (Next xpc1 xrs xm xss) of
+          Stuck \<Rightarrow> (pc, Stuck) | \<comment>\<open> if one step error, stop, it should be impossible \<close>
+          Next xpc1 rs1 m1 ss1 \<Rightarrow> (
+          case find_target_pc_in_l_pc l_jump (uint pc) of
+                      None \<Rightarrow> (pc, Stuck) |
+                      Some npc \<Rightarrow>
+            if rs1 (CR ZF) = 1 then \<comment>\<open> must JUMP \<close>
+             (npc, (Next (nat (fst (l_pc!(unat npc)))) rs1 m1 ss1)) \<comment>\<open> go to the target address in the jited x64 binary \<close>
+            else \<comment>\<open> donot JUMP \<close>
+              (pc+1, Next (xpc1+sz2) rs1 m1 ss1)
+          ))|
+            _ \<Rightarrow> (pc, Stuck)) |
+        Some(sz,Pret_anchor) \<Rightarrow>
+          (case x64_decode (xpc1+sz) l_bin of Some (sz2,Pret) \<Rightarrow>
+          let (pc', ss', caller,fp) = update_stack2 xss in 
+          if find_target_pc_in_l_pc3 l_jump (uint pc) \<noteq> Some (uint pc') then (pc,Stuck) else
+          let rs' = restore_x64_caller xrs caller fp in 
+          let xst_temp = exec_instr Pret sz2 (xpc1+sz) rs' xm ss' in 
+          (case xst_temp of Stuck \<Rightarrow> (pc,Stuck)| Next xpc1 rs1 m1 ss1 \<Rightarrow> 
+            (if xpc1 = (nat (fst (l_pc!(unat pc')))+1) then (pc',Next xpc1 rs1 m1 ss1) else (pc,Stuck) ))|
+          _ \<Rightarrow> (pc,Stuck)) |
+       _  \<Rightarrow>
+          (pc+1, x64_sem num l_bin (Next xpc1 xrs xm xss)))" 
+    apply(unfold flat_bpf_one_step_def Let_def) 
+    using a3 a11 a9 apply(cases "Next xpc1 xrs xm xss",simp_all)
+    subgoal for x11 by fastforce     
+    done
+
+  have c1:"nat ?xpc= xpc1" using a8 c2 a9 by (smt (verit, ccfv_SIG) snd_conv) 
+
+  have "xxst' = perir_step lt (pc,xxst)" using a2 by (metis One_nat_def perir_sem.simps(1) perir_sem.simps(2) split_pairs)
+
+  hence b1:"xxst' = (let (num,off,l) = lt!(unat pc) in 
+       case x64_decode 0 l of 
+      Some(_, Pcall_i _) \<Rightarrow> (let xst_temp = Next 0 xrs xm xss in (off, x64_sem 1 l xst_temp))|
+      Some(sz, Pret_anchor) \<Rightarrow> (let (pc', ss', caller,fp) = update_stack2 xss in 
+          let rs' = restore_x64_caller xrs caller fp in 
+          let xst_temp = Next sz rs' xm ss' in (pc', x64_sem 1 l xst_temp))|      
+      Some(_, Pcmpq_rr src dst) \<Rightarrow> 
+        (let xst_temp = Next 0 xrs xm xss; xst' = x64_sem 1 l xst_temp in
+          case xst' of
+          Next xpc' rs' m' ss'\<Rightarrow>
+            if rs' (CR ZF) = 1 then (off+pc, xst')
+            else (pc+1, xst') |
+          Stuck \<Rightarrow> (pc, Stuck))|      
+      _  \<Rightarrow>
+        (let xst_temp = Next 0 xrs xm xss; xst' = x64_sem num l xst_temp in
+          (pc+1, xst')))" 
+    using perir_step_def b0 a2 a3 apply(cases xxst,simp_all)
+    done
+
+  thus ?thesis
+  proof(cases "\<exists> sz. x64_decode 0 ?l = Some(sz,Pret_anchor)")
+    case True
+    obtain sz where b3_0:"x64_decode 0 ?l = Some(sz,Pret_anchor)" using True by auto
+    hence b3:"xxst' = (let (pc', ss', caller,fp) = update_stack2 xss in 
+          let rs' = restore_x64_caller xrs caller fp in 
+          let xst_temp = Next sz rs' xm ss' in (pc', x64_sem 1 ?l xst_temp))"
+      using b1 True b0 apply(cases "x64_decode (0::nat) ?l",simp_all)
+      apply(cases "lt ! unat pc",simp_all)
+      subgoal for a b c 
+        apply(cases "x64_decode sz c",simp_all)
+        done
+        done
+
+   have b2_1:"?l \<noteq> []"  using a8 apply(unfold well_formed_prog_def) using b0 a4 a7 by blast
+   have "?num >0 " using a8 apply(unfold well_formed_prog_def) using b0 a4 a7 by blast 
+   hence b2_2:"x64_decode 0 ?l \<noteq> None"  apply(cases "x64_decode 0 ?l",simp_all) using True by force
+   hence b2_3:"x64_decode 0 ?l = x64_decode xpc1 l_bin" using b2_2 list_in_list_x64_decode by (metis True add.right_neutral c0 c1) 
+   hence b2_4:"\<exists> num. x64_decode xpc1 l_bin = Some(num,Pret_anchor)" using b2_3 True by auto
+   hence b2_5:"x64_decode  xpc1 l_bin = Some(sz,Pret_anchor)" using b3 b2_3 b3_0 by argo 
+   have b2:"fxst' = (case x64_decode (xpc1+sz) l_bin of Some (sz2,Pret) \<Rightarrow>
+          let (pc', ss', caller,fp) = update_stack2 xss in 
+          if find_target_pc_in_l_pc3 l_jump (uint pc) \<noteq> Some (uint pc') then (pc,Stuck) else
+          let rs' = restore_x64_caller xrs caller fp in 
+          let xst_temp = exec_instr Pret sz2 (xpc1+sz) rs' xm ss' in 
+          (case xst_temp of Stuck \<Rightarrow> (pc,Stuck)| Next xpc1 rs1 m1 ss1 \<Rightarrow> 
+            (if xpc1 = (nat (fst (l_pc!(unat pc')))+1) then (pc',Next xpc1 rs1 m1 ss1) else (pc,Stuck))))" using b2_4 c2 a9 a7 a3
+     using b2_5 c2 
+     apply(cases "x64_decode xpc1 l_bin",simp_all)
+     subgoal for a
+       apply(split if_splits,simp_all)
+         apply(unfold Let_def,simp_all)
+         apply(split if_splits,simp_all)
+         apply(cases "x64_decode (nat (fst (l_pc ! unat pc)) + sz) l_bin",simp_all)
+         subgoal for aa apply(cases aa,simp_all)
+           subgoal for ab b apply(cases b,simp_all)
+         done
+         done
+       done
+     done
+
+   have "\<exists> xpc'' xrs'' xm'' xss'' pc'. fxst' = (pc', Next xpc'' xrs'' xm'' xss'')" using a9
+     by (metis eq_snd_iff outcome.exhaust) 
+   then obtain xpc'' xrs'' xm'' xss'' pc' where b3_0:"fxst' = (pc', Next xpc'' xrs'' xm'' xss'')" by auto
+   have b3_1:"Next xpc'' xrs'' xm'' xss'' \<noteq> Stuck" using b3_0 a9 by blast
+   hence b4:"\<exists> sz2. x64_decode (xpc1+sz) l_bin = Some (sz2,Pret)" using a9 b2 b3_0 
+     apply(cases "x64_decode (xpc1 + sz) l_bin",simp_all) 
+     sorry
+
+
+   then obtain sz2 where "x64_decode (xpc1+sz) l_bin = Some (sz2,Pret)" by auto
+   hence b4_1:"fxst' = (let (pc', ss', caller,fp) = update_stack2 xss in 
+          if find_target_pc_in_l_pc3 l_jump (uint pc) \<noteq> Some (uint pc') then (pc,Stuck) else
+          let rs' = restore_x64_caller xrs caller fp in 
+          let xst_temp = exec_instr Pret sz2 (xpc1+sz) rs' xm ss' in 
+          (case xst_temp of Stuck \<Rightarrow> (pc,Stuck)| Next xpc1 rs1 m1 ss1 \<Rightarrow> 
+            (if xpc1 = (nat (fst (l_pc!(unat pc')))+1) then (pc',Next xpc1 rs1 m1 ss1) else (pc,Stuck))))"
+     using b2 apply(cases "update_stack2 xss",simp_all)
+        done
+
+   let "?ss'" = "(fst(snd(update_stack2 xss)))"
+   let "?rs'" = "(restore_x64_caller xrs (fst(snd(snd(update_stack2 xss)))) (snd(snd(snd(update_stack2 xss)))))"
+   let "?pc'" = "fst (update_stack2 xss)"
+
+      have b4_2:"find_target_pc_in_l_pc3 l_jump (uint pc) = Some (uint (?pc'))" using b4_1 a9
+       apply(cases "update_stack2 xss",simp_all)
+       subgoal for a b c d 
+         apply(split if_splits,simp_all)
+          done
+        done
+      have b4_3:"exec_instr Pret sz2 (xpc+sz) ?rs' xm ?ss' \<noteq> Stuck" 
+        using b4_1 b4_2 apply(unfold Let_def,simp_all) apply(cases "update_stack2 xss",simp_all)
+        subgoal for a b c d
+          using a9 exec_instr_def by force 
+        done
+      hence "\<exists> xpc1 xrs1 xss1 xm1. exec_instr Pret sz2 (xpc+sz) ?rs' xm ?ss' = Next xpc1 xrs1 xss1 xm1"
+        by (meson outcome.exhaust) 
+  (*    then obtain xpc1 xrs1 xss1 xm1 where b4_4:"exec_instr Pret sz2 (xpc+sz) ?rs' xm ?ss' = Next xpc1 xrs1 xss1 xm1" by auto
+
+          hence c0_6:"Next xpc1 xrs1 xss1 xm1 = Next xpc'' xrs'' xm'' xss''"
+          using c0 c0_2 cn c0_3 apply(unfold Let_def,simp_all) 
+          by(cases "update_stack2 xss",simp_all)
+      
+      have c0_4:"exec_instr Pret sz2 (xpc+sz) ?rs' xm ?ss' = (
+          let nsp =  (?rs' (IR SP)) + (u64_of_memory_chunk M64) in
+            case Mem.loadv M64 xm (Vptr sp_block nsp) of
+            None \<Rightarrow> Stuck |
+            Some ra \<Rightarrow> (
+              case ra of
+              Vlong v \<Rightarrow> let rs1 = ?rs'#(IR SP) <- nsp in
+                          Next (unat v) rs1 xm ?ss' |
+              _ \<Rightarrow> Stuck)
+        )" using exec_instr_def by (simp add: exec_ret_def) 
+
+      hence "\<exists> v. Mem.loadv M64 xm (Vptr sp_block ((?rs' (IR SP)) + (u64_of_memory_chunk M64))) = Some (Vlong v)"
+        using c0_3 c0_2
+        by (smt (verit, ccfv_SIG) option.case_eq_if option.collapse val.case(1) val.case(2) val.case(3) val.case(4) val.case(6) val.exhaust) 
+
+      then obtain v where c0_5:"Mem.loadv M64 xm (Vptr sp_block ((?rs' (IR SP)) + (u64_of_memory_chunk M64))) = Some (Vlong v)" by auto
+      
+      hence c0_7:"exec_instr Pret sz2 (xpc+sz) ?rs' xm ?ss' = Next (unat v) (?rs'#(IR SP) <- ((?rs' (IR SP)) + (u64_of_memory_chunk M64))) xm ?ss'" 
+        using c0_4 Let_def by simp
+      hence c1:"snd fxst' = Next (unat v) (?rs'#(IR SP) <- ((?rs' (IR SP)) + (u64_of_memory_chunk M64))) xm ?ss'" 
+        using c0_6 c0_3 a1 by argo 
+*)
+   have "JITFlattern_def.match_state xxst' fxst'" 
+     using  a6 a9 b2 b3 by(unfold JITFlattern_def.match_state_def match_state1_def Let_def update_stack2_def,simp_all) 
+    then show ?thesis by simp
+  next
+    case False
+    have b2:"\<not>(\<exists> num. x64_decode 0 ?l = Some(num,Pret_anchor))" using False by simp
+
+    then show ?thesis   
+    proof(cases "(\<exists> d num. x64_decode 0 ?l = Some(num, Pcall_i d))")
+      case True
+      have b3:"(\<exists> d num. x64_decode 0 ?l = Some(num, Pcall_i d))" using True by simp
+      then obtain sz d where b3_0:"x64_decode 0 ?l = Some(sz, Pcall_i d)" by auto
+      have b4:"xxst' = (?off, (x64_sem 1 ?l (Next 0 xrs xm xss)))" 
+        using True b1 b0 b2 apply(cases "x64_decode 0 ?l",simp_all)
+        subgoal for a
+          apply(cases "lt ! unat pc",simp_all)
+          subgoal for aa b c
+            apply(cases a,simp_all)
+            subgoal for ab ba apply(cases ba,simp_all)
+              done
+            done
+          done
+        done
+              
+      have b2_1:"?l \<noteq> []"  using a8 apply(unfold well_formed_prog_def) using b0 a4 a7 by blast
+      have "?num >0 " using a8 apply(unfold well_formed_prog_def) using b0 a4 a7 by blast 
+      hence b2_2:"x64_decode 0 ?l \<noteq> None" apply(cases "x64_decode 0 ?l",simp_all) using b3 by force 
+
+      
+      (*hence "\<forall> n. \<not> (x64_bin_is_sequential n ?l 0)" using x64_bin_is_sequential_x64_decode_pcall_false by blast*)
+      have d3_1:"x64_decode 0 ?l = x64_decode xpc1 l_bin " 
+        using list_in_list_x64_decode c0 by (metis add.right_neutral c1 b3) 
+
+      have d3_2:"x64_decode xpc1 l_bin = Some(sz, Pcall_i d)"
+        using b3_0 d3_1 by auto 
+
+      hence d3:"fxst' =  (case x64_decode (xpc1+sz) l_bin of Some (sz2,Pjcc _ _) \<Rightarrow>
+            (case x64_sem ?num l_bin (Next xpc1 xrs xm xss) of
+            Stuck \<Rightarrow> (pc, Stuck) | \<comment>\<open> if one step error, stop, it should be impossible \<close>
+            Next xpc' rs1 m1 ss1 \<Rightarrow> (
+              case find_target_pc_in_l_pc l_jump (uint pc) of
+                None \<Rightarrow> (pc, Stuck) |
+                Some npc \<Rightarrow>
+              if rs1 (CR ZF) = 1 then \<comment>\<open> must JUMP \<close>
+                ((npc, (Next (nat (fst (l_pc!(unat npc)))) rs1 m1 ss1))) \<comment>\<open> go to the target address in the jited x64 binary \<close>
+              else \<comment>\<open> donot JUMP \<close>
+                (pc+1, (Next (xpc'+sz2) rs1 m1 ss1))
+            )))"
+        using d3_2 a9 c2 a7 a3 a11 c1 apply(split if_splits,simp_all) sorry
+        
+
+      thus ?thesis
+        proof(cases "find_target_pc_in_l_pc l_jump (uint pc) \<noteq> None")
+          case True
+          have "\<exists> npc. find_target_pc_in_l_pc l_jump (uint pc) = Some npc" using True by simp
+          then obtain npc where d5_1:"find_target_pc_in_l_pc l_jump (uint pc) = Some npc" by auto
+          have d5_2:"distinct (map fst [])" by simp
+          have d5_4:"is_increase_list [] []" using is_increase_list_empty by blast 
+          hence d5:"npc = ?off" using a1 b0 d5_2 init_second_layer_def a7 b3 d5_4 d5_1 flattern_jump_index_2
+            by (smt (verit, ccfv_threshold) int_ops(1) list.size(3)) 
+
+          have d6_0:"fxst' = (case x64_sem 1 l_bin fxst of  Next xpc' rs' m' ss' \<Rightarrow> (?off, (x64_sem 1 l_bin (Next (nat (fst (l_pc!(unat npc)))) rs' m' ss'))) )" using d5 d3 d5_1 sorry
+
+          hence d6: "JITFlattern_def.match_state xxst' fxst'" 
+            using b4 d5 d3 True JITFlattern_def.match_state_def match_state1_def a9 a6 sorry
+          then show ?thesis by simp             
+        next
+          case False
+          have "find_target_pc_in_l_pc l_jump (uint pc) = None" using False by simp
+           hence "fxst' = (pc,Stuck)" using d3 by simp
+          then show ?thesis using a9 by auto
+        qed
+    next
+      case False
+      have b5:"(\<not> (\<exists> num. x64_decode 0 ?l = Some(num,Pret_anchor))) \<and> (\<not>(\<exists> num d. x64_decode 0 ?l = Some(num, Pcall_i d)))" using False b2 by simp
+      hence bn_1:"?l \<noteq> []" using a8 apply(unfold well_formed_prog_def) using b0 a4 a7 by blast
+      have bn_2:"?num >0 " using a8 apply(unfold well_formed_prog_def) using b0 a4 a7 by blast 
+
+      have c3_0:"list_in_list ?l xpc1 l_bin" using c0 c1 by simp         
+      have c3:"l_bin!xpc1 = ?l!0" using c3_0 bn_1 by (metis list.collapse list_in_list.simps(2) nth_Cons_0)
+      then show ?thesis      
+      proof(cases "(\<exists> num src dst. x64_decode 0 ?l = Some(num, Pcmpq_rr src dst))")
+        
+        case True
+        
+        hence d0:"xxst' = (let xst_temp = Next 0 xrs xm xss; xst' = x64_sem 1 ?l xst_temp in
+          case xst' of
+          Next xpc' rs' m' ss'\<Rightarrow>
+            if rs' (CR ZF) = 1 then (?off+pc, xst')
+            else (pc+1, xst') |
+          Stuck \<Rightarrow> (pc, Stuck) )" using True b1 b0 b5 apply(cases "x64_decode 0 ?l",simp_all)
+        subgoal for a
+          apply(cases "lt ! unat pc",simp_all)
+          subgoal for aa b c
+            apply(cases a,simp_all)
+            subgoal for ab ba apply(cases ba,simp_all)
+              subgoal for x21a
+                by (metis fst_conv snd_conv) 
+              done
+            done
+          done
+        done
+        
+       have d1_1:"\<exists> sz src dst. x64_decode xpc1 l_bin = Some(sz, Pcmpq_rr src dst)" 
+          using list_in_list_x64_decode c3_0 True by fastforce 
+        then obtain sz src dst where d1_0:"x64_decode xpc1 l_bin = Some(sz, Pcmpq_rr src dst)" by auto
+        hence d1:"fxst' = (case x64_decode (xpc1+sz) l_bin of Some (sz2,Pjcc _ _) \<Rightarrow>
+          (case x64_sem (snd (l_pc!(unat pc))) l_bin (Next xpc1 xrs xm xss) of
+          Stuck \<Rightarrow> (pc, Stuck) | \<comment>\<open> if one step error, stop, it should be impossible \<close>
+          Next xpc1 rs1 m1 ss1 \<Rightarrow> (
+          case find_target_pc_in_l_pc l_jump (uint pc) of
+                      None \<Rightarrow> (pc, Stuck) |
+                      Some npc \<Rightarrow>
+            if rs1 (CR ZF) = 1 then \<comment>\<open> must JUMP \<close>
+             (npc, (Next (nat (fst (l_pc!(unat npc)))) rs1 m1 ss1)) \<comment>\<open> go to the target address in the jited x64 binary \<close>
+            else \<comment>\<open> donot JUMP \<close>
+              (pc+1, Next (xpc1+sz2) rs1 m1 ss1)
+          ))|
+            _ \<Rightarrow> (pc, Stuck))" using True a0 c2 a7 a9 c1 by auto 
+        hence d1_2:"\<exists> sz2 cond d. x64_decode (xpc1+sz) l_bin = Some (sz2,Pjcc cond d)" 
+          using a9 apply(cases "x64_decode (xpc1+sz) l_bin",simp_all)
+          subgoal for a apply(cases a,simp_all)
+            subgoal for aa b by(cases b,simp_all)
+            done
+          done
+        then obtain sz2 cond d where d1_3:"x64_decode (xpc1+sz) l_bin = Some (sz2,Pjcc cond d)" by auto
+
+        have d4:"(snd (l_pc!(unat pc))) = ?num"
+          by (metis (mono_tags, lifting) a1 a7 b0 flattern_num)      
+        have b7_0:"\<exists> num src dst. x64_decode 0 ?l = Some(num, Pcmpq_rr src dst)" using True bn_1 by simp
+        have b7:"?num = 1" using a10 b7_0 by (metis a7 b0 jit_prog_prop4)  
+
+        have "\<exists> fxst1. fxst1 = x64_sem 1 l_bin (Next xpc1 xrs xm xss)" by fastforce
+        then obtain fxst1 where d2_0:"fxst1 = x64_sem 1 l_bin (Next xpc1 xrs xm xss)" by auto
+        have "\<exists> xxst1. xxst1 = x64_sem 1 ?l (Next 0 xrs xm xss)" by fastforce
+        then obtain xxst1 where d2_1:"xxst1 = x64_sem 1 ?l (Next 0 xrs xm xss)" by auto
+        have d2_5_1:"xxst1 \<noteq> Stuck" using a6 d1 d2_1 d4 d0 by force
+        hence d2_5:"x64_decode 0 ?l \<noteq> None" using d2_1 by(cases "x64_decode 0 ?l",simp_all)
+                
+        hence d2_2:"fxst1 = (case x64_decode xpc1 l_bin of
+          None \<Rightarrow> Stuck |
+          Some (sz, ins) \<Rightarrow>
+            x64_sem 0 l_bin (exec_instr ins sz xpc1 xrs xm xss)
+          )" using d2_0 by simp
+        have d2_3_1:"fxst1 \<noteq> Stuck" using a9 d1 d2_0 b0 d4 d1_2 d1_3 b7 d1_0 sorry
+        hence d2_3:"x64_decode xpc1 l_bin \<noteq> None" using d2_2 by(cases "x64_decode xpc1 l_bin",simp_all)
+        hence d2_4:"fxst1 = (case x64_decode xpc1 l_bin of Some (sz, ins) \<Rightarrow> (exec_instr ins sz xpc1 xrs xm xss))" 
+          using d2_2 by force
+
+      
+        have d2_6:"xxst1 = (case x64_decode 0 ?l of Some (sz, ins) \<Rightarrow> (exec_instr ins sz 0 xrs xm xss))"
+          using b7 d2_1 d2_5 by force 
+        
+        have d2_7:"x64_decode 0 ?l = x64_decode xpc1 l_bin" using list_in_list_x64_decode d2_3 d2_5 c3_0 by fastforce 
+        have "\<exists> sz ins. x64_decode 0 ?l = Some (sz, ins)" using d2_5 by simp
+        then obtain sz ins where "x64_decode 0 ?l = Some (sz, ins)" by auto
+        hence d2_8:"xxst1 = (exec_instr ins sz 0 xrs xm xss)" using d2_6 by simp
+        hence d2_9:"fxst1 =(exec_instr ins sz xpc1 xrs xm xss)" using d2_0 d2_1 d2_6 d2_4 d2_7
+          by (metis \<open>x64_decode (0::nat) (snd (snd ((lt::(nat \<times> 64 word \<times> 8 word list) list) ! unat (pc::64 word)))) = Some (sz::nat, ins::instruction)\<close> case_prod_conv option.simps(5)) 
+        have d2:"match_state1 fxst1 xxst1" using match_state1_prop d2_3_1 d2_5_1 d2_8 d2_9 by blast
+          
+          have d3:"\<exists> xpc' xrs1 xm1 xss1. Next xpc' xrs1 xm1 xss1 = fxst1" 
+            using d2 match_state1_def by (smt (verit, ccfv_threshold) outcome.exhaust outcome.simps(5)) 
+          then obtain xpc' xrs1 xm1 xss1 where d4_0:"Next xpc' xrs1 xm1 xss1 = fxst1" by auto
+          have "\<exists> xpc''. Next xpc'' xrs1 xm1 xss1 = xxst1" 
+            using d3 match_state1_def d4_0 by (smt (verit, ccfv_SIG) d2 outcome.exhaust outcome.simps(4) outcome.simps(5))
+          then obtain xpc'' where d4_1:"Next xpc'' xrs1 xm1 xss1 = xxst1" by auto
+          
+          thus ?thesis
+          proof(cases "xrs1 (CR ZF) = 1")
+            case True
+            have d5_0: "xrs1 (CR ZF) = 1" using True by auto
+            thus ?thesis
+            proof(cases "find_target_pc_in_l_pc l_jump (uint pc) \<noteq> None")
+              case True
+                have "\<exists> npc. find_target_pc_in_l_pc l_jump (uint pc) = Some npc" using True by simp
+                then obtain npc where d5_1:"find_target_pc_in_l_pc l_jump (uint pc) = Some npc" by auto
+                have d5_2:"distinct (map fst [])" by simp
+                have d5_4:"is_increase_list [] []" using is_increase_list_empty by blast 
+                hence d5:"npc = ?off+pc" using a1 a4 b0 a7 flattern_jump_index_1 init_second_layer_def d5_2 d5_1 b7_0
+                  by (metis (mono_tags, lifting) Abs_fnat_hom_0 add_0 int_ops(1) list.size(3))
+                                                 
+                have d6_0:"fxst' =  (npc, (Next (nat (fst (l_pc!(unat npc)))) xrs1 xm1 xss1))" 
+                  using d5_0 d5_1 True d4_0 d1 d2_0 d4 d1_2 sorry
+                have d6_1:"xxst' = (?off+pc, xxst1)"
+                  by (smt (verit, ccfv_threshold) d0 d2_1 d4_1 d5_0 outcome.simps(4)) 
+
+                have "JITFlattern_def.match_state fxst' xxst'" 
+                  using d6_0 d6_1 JITFlattern_def.match_state_def d4_1 d5 match_state1_def by auto
+                then show ?thesis using JITFlattern_def.match_state_def d6_0 d6_1 match_state1_def \<open>\<And>thesis::bool. (\<And>xpc''::nat. Next xpc'' (xrs1::preg \<Rightarrow> 64 word) (xm1::nat \<Rightarrow> int \<Rightarrow> 8 word option) (xss1::stack_state) = (xxst1::outcome) \<Longrightarrow> thesis) \<Longrightarrow> thesis\<close> by fastforce 
+               next
+                 case False
+                 have "find_target_pc_in_l_pc l_jump (uint pc) = None" using False by simp
+                 hence "fxst' = (pc,Stuck)" using a9 d1 d2_0 d4 d4_0 d5_0 d1_2 sorry
+                   
+                then show ?thesis using a9 by auto
+              qed
+            next
+              case False
+              have d5_0:"xrs1 (CR ZF) \<noteq> 1" using False by simp
+              have d5_1:"xxst' = (pc+1, xxst1)" by (smt (verit) d0 d2_1 d4_1 d5_0 outcome.simps(4)) 
+              have d5_2:"fxst' = (pc+1, fxst1)" 
+                using d5_0 d1 d2_0 d4 d4_0 d1_2 sorry
+            then show ?thesis using d5_1 d5_2 JITFlattern_def.match_state_def d2 d3 d4_1 by force 
+        qed
+
+      next
+        case False
+        have b6:"(\<not>(\<exists> num. x64_decode 0 ?l = Some(num,Pret_anchor))) \<and> (\<not>(\<exists> num d. x64_decode 0 ?l = Some(num, Pcall_i d))) \<and> (\<not> (\<exists> num src dst. x64_decode 0 ?l = Some(num, Pcmpq_rr src dst)))" 
+          using b5 False by force 
+          have d0:"xxst' = (let xst_temp = Next 0 xrs xm xss; xst' = x64_sem ?num ?l xst_temp in
+          (pc+1, xst'))" using b6 b0 b1 apply(cases "x64_decode 0 ?l",simp_all)
+            apply(cases "lt ! unat pc",simp_all)
+            subgoal for a apply(cases "lt ! unat pc",simp_all)
+              subgoal for aa b c
+                apply(cases a,simp_all)
+                subgoal for ab ba apply(cases ba,simp_all)
+                  done
+                done
+              done
+            done
+          hence bn_0:"x64_decode 0 ?l \<noteq> None" using d0 a6 bn_2 apply(cases "x64_decode 0 ?l",simp_all)
+            by (smt (verit) Suc_diff_1 option.simps(4) x64_sem.simps(3))
+          hence "x64_decode 0 ?l \<noteq> Some(1,Pret_anchor) \<and> (\<forall> d. x64_decode 0 ?l \<noteq> Some(5, Pcall_i d)) \<and> (\<forall> src dst. x64_decode 0 ?l \<noteq> Some(3, Pcmpq_rr src dst))"
+            using  bn_1 b6 by simp
+
+          have "(\<not>(\<exists> num. x64_decode xpc1 l_bin = Some(num,Pret_anchor))) \<and> (\<not>(\<exists> num d. x64_decode xpc1 l_bin = Some(num, Pcall_i d))) \<and> (\<not> (\<exists> num src dst. x64_decode xpc1 l_bin = Some(num, Pcmpq_rr src dst)))" 
+            using b6 list_in_list_x64_decode bn_0 c3_0 by fastforce
+          hence c4:"fxst' = (let num = snd (l_pc!(unat pc)) in (pc+1, x64_sem num l_bin (Next xpc1 xrs xm xss)))"
+            using c2 b6  a1 a7 add.right_neutral c1 init_second_layer_def l_pc_length_prop a9 a9 c2 snd_conv
+          apply(cases "x64_decode xpc1 l_bin",simp_all)
+            apply(cases "lt ! unat pc",simp_all)
+            subgoal for a apply(cases "lt ! unat pc",simp_all)
+              subgoal for aa
+                apply(split if_splits,simp_all)
+                done
+              done
+            subgoal for a
+              apply(split if_splits,simp_all)
+                apply(cases a,simp_all)                
+                subgoal for aa b apply(cases b,simp_all)
+                  done
+                done
+              done           
+           
+          have c5_1:"l_pc \<noteq> []"  using a1 a4 apply(unfold init_second_layer_def) using num_corr by fastforce 
+
+          have c5:"fxst' = (pc+1, x64_sem ?num l_bin (Next xpc1 xrs xm xss))"using b0 c5_1 a1 init_second_layer_def c4 a6 a7
+            by (metis (mono_tags, lifting) flattern_num)
+
+          hence c6:"x64_bin_is_sequential (length ?l) ?l 0" using a10 x64_bin_is_sequential_x64_decode2 b6 a7 b0 bn_0 by metis
+          
+          have cn:"match_state1 (snd xxst') (snd fxst')" using c5 d0 c3_0 list_in_list_prop3 c6 a6 a9 by (metis add.right_neutral snd_conv) 
+            
+          have "fst fxst' = pc+1" using c5 by auto
+          moreover have d2:"fst xxst' = pc+1" using d0 by auto
+          hence "fst xxst' = fst fxst'" using calculation by presburger 
+          hence "JITFlattern_def.match_state xxst' fxst'" using cn JITFlattern_def.match_state_def match_state1_def match_mem_def
+            apply(cases "snd xxst'",simp_all)
+            apply(cases "snd fxst'",simp_all)
+            by (simp add: case_prod_beta')                    
+          then show ?thesis by (simp add: c5 d0) 
+        qed
+      qed
+    qed
+  qed
 
 lemma flat_bpf_sem_induct_aux1:
  "flat_bpf_sem (m+n) x64_prog xst = xst'\<Longrightarrow> 
@@ -437,26 +981,32 @@ next
   then obtain next_s pc' where b0:"next_s = perir_sem 1 lt (pc,xxst)" by auto
   have "\<exists> next_f. flat_bpf_sem 1 prog (pc,fxst) = next_f" by blast
   then obtain next_f where b1:"flat_bpf_sem 1 prog (pc,fxst) = next_f" by simp
-  (*have b2:"xrs1 = xrs \<and> xm = xm1 \<and> xss = xss1" using match_state_def assm3 assm7 assm6
-    apply(cases "fxst",simp_all)
-    done*)
   have a0:"perir_sem n lt next_s = xxst'" using x64_sem1_induct_aux3 assm2 b0
     using Suc.prems(3) by presburger 
   have "\<exists> pc' xrs1 xpc1 m1 xss1. (pc', Next xrs1 xpc1 m1 xss1) = next_s" using assm4 a0 intermediate_step_is_ok
     by (metis outcome.exhaust prod.collapse zero_le) 
   then obtain pc' xrs1 xpc1 m1 xss1 where a1:"(pc', Next xrs1 xpc1 m1 xss1) = next_s" by auto
                                                                                                             
-  (*have "\<exists> pc'' xrs1' xpc1' m1' xss1'. (pc'', Next xrs1' xpc1' m1' xss1') = next_f" using assm8 intermediate_step_is_ok3 b1
-    by (metis Suc.prems(9) assm0 bot_nat_0.extremum flat_bpf_sem_induct_aux2 outcome.distinct(1) prod.exhaust_sel) *)
   have c0_1:"snd next_f \<noteq> Stuck" using assm8 intermediate_step_is_ok3 b1
     by (metis assm0 bot_nat_0.extremum flat_bpf_sem_induct_aux2 outcome.distinct(1) prod.exhaust_sel) 
 
-  hence"(unat pc < length (fst(snd prog)) \<and> unat pc \<ge> 0)" using b1 assm8 
-    using One_nat_def case_prod_conv flat_bpf_one_step_def flat_bpf_sem.simps(1) flat_bpf_sem.simps(2) 
-        intermediate_step_is_ok3 linorder_not_less outcome.simps(4) prod.collapse split_pairs zero_order(1)
-    by (smt (verit)) 
+  have c0_2:"\<exists> xpc1 xrs xm xss. Next xpc1 xrs xm xss = fxst" 
+    using assm6 assm3 JITFlattern_def.match_state_def apply(cases xxst,simp_all) 
+    subgoal for x11 by(cases fxst,simp_all) done
+  have c0_3:"(unat pc < length (fst(snd prog)) \<and> unat pc \<ge> 0)" 
+  proof(rule ccontr)
+    assume assm:"\<not> (unat pc < length (fst(snd prog)) \<and> unat pc \<ge> 0)"
+    have "snd next_f = snd (let pair = flat_bpf_one_step prog (pc, fxst) in
+    flat_bpf_sem 0 prog pair)" using b1 by auto 
+    hence "snd next_f = snd (flat_bpf_one_step prog (pc, fxst))"
+      by (metis flat_bpf_sem.simps(1) prod.collapse) 
+    hence "snd next_f = Stuck" 
+      using flat_bpf_one_step_def c0_2 assm apply(cases fxst,simp_all)
+      subgoal for x11 x12 x13 x14 by(cases prog,simp_all) done
+    thus "False" using c0_1 by blast
+  qed
 
-  hence c0:"(unat pc < length lt \<and> unat pc \<ge> 0)" using l_pc_length_prop  init_second_layer_def assm1
+  hence c0:"(unat pc < length lt \<and> unat pc \<ge> 0)" using l_pc_length_prop init_second_layer_def assm1
     by (metis add.right_neutral list.size(3) prod.collapse) 
   have bn:"JITFlattern_def.match_state next_s next_f"
     using one_step_equiv_layer1 b1 assm1 b0 assm3 assm5 assm6 a1 c0 assm8 c0_1 assm7 assm9
@@ -473,14 +1023,7 @@ next
 
   hence "JITFlattern_def.match_state xxst' fxst'" 
     using a0 a1 a2 Suc bn c1 assm5 assm4 by metis
-  then show ?case by simp
+  then show ?case by blast
 qed
-
-
-
-
-
-
-
 
 end
