theory/JITFlattern_aux_well_formed.thy
@@ -38,16 +38,8 @@ per_jit_shift_arsh_reg64_def per_jit_load_reg64_def  per_jit_store_reg64_def per
     done
   done
 
-(*lemma jit_prog_prop2:"per_jit_ins ins = Some (num,off,l_bin0) \<Longrightarrow> \<exists> src dst. x64_decode 0 l_bin0 = Some(3, Pcmpq_rr src dst) \<Longrightarrow> l_bin0\<noteq>[] \<Longrightarrow> num = 1"*)
-lemma jit_prog_prop3:
-  "jitper insns = Some lt \<Longrightarrow> 
-  lt \<noteq> [] \<Longrightarrow>
-  lt!(unat pc) = (num,off,l_bin0) \<Longrightarrow> 
-  unat pc < length lt \<and> unat pc \<ge> 0 \<Longrightarrow> 
-  num > 0"
-  sorry
 
-lemma jit_prog_prop2:"per_jit_ins ins = Some (num,off,l_bin0) \<Longrightarrow> \<exists> src dst. x64_decode 0 l_bin0 = Some(3, Pcmpq_rr src dst) \<Longrightarrow>  num = 1"
+lemma jit_prog_prop2:"per_jit_ins ins = Some (num,off,l_bin0) \<Longrightarrow> \<exists> num src dst. x64_decode 0 l_bin0 = Some(num, Pcmpq_rr src dst) \<Longrightarrow>  num = 1"
   using x64_encode_decode_consistency 
   apply(unfold per_jit_ins_def,simp_all)
 apply(unfold per_jit_load_reg64_def per_jit_add_reg64_1_def per_jit_add_imm64_1_def  per_jit_sub_reg64_1_def per_jit_mov_reg64_1_def 
@@ -573,7 +565,8 @@ apply(subgoal_tac "x64_decode 0 l_bin0 = Some (1,Ppushl_r RCX)")
                      apply (meson list_in_list_concat list_in_list_prop)
       done
     done
-  done
+  sorry
+
 
 
 
@@ -581,7 +574,7 @@ lemma jit_prog_prop4:
   "jitper insns = Some lt \<Longrightarrow> 
   lt!(unat pc) = (num,off,l_bin0) \<Longrightarrow> 
   unat pc < length lt \<and> unat pc \<ge> 0 \<Longrightarrow> 
-  \<exists> src dst. x64_decode 0 l_bin0 = Some(3, Pcmpq_rr src dst) \<Longrightarrow> 
+  \<exists> num src dst. x64_decode 0 l_bin0 = Some(num, Pcmpq_rr src dst) \<Longrightarrow> 
   num = 1"
 
   proof(induct lt arbitrary:insns pc num off l_bin0)
@@ -592,7 +585,7 @@ lemma jit_prog_prop4:
     assume assm0: "jitper insns = Some (a#lt)" and
       assm1:"(a#lt)!(unat pc) = (num,off,l_bin0)" and
       assm2:"unat pc < length (a#lt) \<and> unat pc \<ge> 0" and
-      assm3:"\<exists> src dst. x64_decode 0 l_bin0 = Some(3, Pcmpq_rr src dst)"
+      assm3:"\<exists> num src dst. x64_decode 0 l_bin0 = Some(num, Pcmpq_rr src dst)"
     have a0:"unat pc = 0 \<or> unat pc \<ge> 1" by auto
     show ?case
     proof (cases "unat pc = 0")
@@ -601,7 +594,7 @@ lemma jit_prog_prop4:
         by (smt (verit) True aux5 is_none_code(2) is_none_simps(1) jitper.elims length_greater_0_conv list.simps(3) nth_Cons_0 option.inject option.split_sel) 
       then obtain ins where b1:"per_jit_ins ins = Some a" by auto
       then show ?thesis using jit_prog_prop2
-        using True assm3 local.Cons(3) by auto 
+        using True assm3 local.Cons(3) by auto
     next
       case False
       let "?pc" = "unat pc -1"
@@ -622,46 +615,6 @@ lemma jit_prog_prop4:
       qed     
     qed
 
-lemma "jitper insns = Some lt \<Longrightarrow> lt \<noteq> [] \<Longrightarrow> well_formed_prog1 lt"
-  using jit_prog_prop3 well_formed_prog1_def sorry
 
-
-
-(*
-lemma jit_prog_prop1:"x64_encode ins \<noteq> undefined \<Longrightarrow>  x64_encode ins \<noteq> []"
-  apply(unfold x64_encode_def)
-  apply(cases ins,simp_all)
-  subgoal for x7 
-    apply(unfold construct_rex_to_u8_def Let_def,simp_all)
-    done
-  subgoal for x8
-    apply(unfold construct_rex_to_u8_def Let_def,simp_all)
-    done
-  subgoal for x111 x112
-apply(unfold construct_rex_to_u8_def Let_def,simp_all)
-    done
-  subgoal for x151 x152 x153
-    apply(cases x151,simp_all)
-    subgoal for x1 x2 x3 
-      apply(cases x1,simp_all) 
-      subgoal for a apply(cases x2,simp_all)
-         apply(unfold construct_rex_to_u8_def Let_def,simp_all)
-        sorry
-      done
-    done
-  subgoal for x201 x202 x203
-    apply(cases x202,simp_all) 
-    subgoal for x1 x2 x3
-      apply(cases x1,simp_all) 
-      subgoal apply(cases x2,simp_all) 
-         apply(unfold construct_rex_to_u8_def Let_def,simp_all)
-         apply(cases x203,simp_all) 
-        sorry
-    done
-  done
-*)
-
-(*lemma "jitper insns = Some lt \<Longrightarrow> insns \<noteq> [] \<Longrightarrow> lt \<noteq> []"
-  using jit_prog_prop3 *)
 
 end
